@prefix ai: <https://spdx.org/rdf/v3/AI/> .
@prefix build: <https://spdx.org/rdf/v3/Build/> .
@prefix core: <https://spdx.org/rdf/v3/Core/> .
@prefix dataset: <https://spdx.org/rdf/v3/Dataset/> .
@prefix expandedlicensing: <https://spdx.org/rdf/v3/ExpandedLicensing/> .
@prefix ns0: <http://www.w3.org/2003/06/sw-vocab-status/ns#> .
@prefix owl: <http://www.w3.org/2002/07/owl#> .
@prefix rdf: <http://www.w3.org/1999/02/22-rdf-syntax-ns#> .
@prefix rdfs: <http://www.w3.org/2000/01/rdf-schema#> .
@prefix security: <https://spdx.org/rdf/v3/Security/> .
@prefix sh: <http://www.w3.org/ns/shacl#> .
@prefix simplelicensing: <https://spdx.org/rdf/v3/SimpleLicensing/> .
@prefix software: <https://spdx.org/rdf/v3/Software/> .
@prefix xsd: <http://www.w3.org/2001/XMLSchema#> .

core:Organization a owl:Class,
        sh:NodeShape ;
    rdfs:comment "An Organization is a group of people who work together in an organized way for a shared purpose." ;
    rdfs:subClassOf core:Agent ;
    ns0:term_status "Stable" .

core:Person a owl:Class,
        sh:NodeShape ;
    rdfs:comment "A Person is an individual human being." ;
    rdfs:subClassOf core:Agent ;
    ns0:term_status "Stable" .

core:SoftwareAgent a owl:Class,
        sh:NodeShape ;
    rdfs:comment "A SoftwareAgent is a software program that is given the authority (similar to a user's authority) to act on a system." ;
    rdfs:subClassOf core:Agent ;
    ns0:term_status "Stable" .

core:SpdxDocument a owl:Class,
        sh:NodeShape ;
    rdfs:comment """An SpdxDocument assembles a collection of Elements under a common string, the name of the document.
Commonly used when representing a unit of transfer of SPDX Elements.
External property restriction on /Core/Element/name: minCount: 1""" ;
    rdfs:subClassOf core:Bundle ;
    ns0:term_status "Stable" .

core:prefix a owl:DatatypeProperty ;
    rdfs:comment "A prefix is a substitute for a URI." ;
    rdfs:range xsd:string ;
    ns0:term_status "Stable" .

expandedlicensing:CustomLicense a owl:Class,
        sh:NodeShape ;
    rdfs:comment """A CustomLicense represents a License that is not listed on the SPDX License
List at https://spdx.org/licenses, and is therefore defined by an SPDX data
creator.""" ;
    rdfs:subClassOf expandedlicensing:License ;
    ns0:term_status "Stable" .

expandedlicensing:CustomLicenseAddition a owl:Class,
        sh:NodeShape ;
    rdfs:comment """A CustomLicenseAddition represents an addition to a License that is not listed
on the SPDX Exceptions List at https://spdx.org/licenses/exceptions-index.html,
and is therefore defined by an SPDX data creator.

It is intended to represent additional language which is meant to be added to
a License, but which is not itself a standalone License.""" ;
    rdfs:subClassOf expandedlicensing:LicenseAddition ;
    ns0:term_status "Stable" .

expandedlicensing:additionComment a owl:DatatypeProperty ;
    rdfs:comment """An additionComment for a LicenseAddition describes general factual information
about the LicenseAddition. It should not contain information (or links to
information) that includes any kind of interpretation about the meaning or
effect of the License, even if written by the license addition's author.

Examples of information for an additionComment may include the following:

* If the LicenseAddition's identifier is deprecated, it may briefly explain the
  reason for deprecation.
* It may include the date of release, if identified, for LicenseAdditions with
  multiple versions.
* It may include links to other official language translations for the
  LicenseAddition.
* It may include a reference to the License(s) with which this LicenseAddition
  is typically used.""" ;
    rdfs:range xsd:string ;
    ns0:term_status "Stable" .

expandedlicensing:additionId a owl:DatatypeProperty ;
    rdfs:comment """An additionId contains a human-readable, short-form identifier for a
LicenseAddition. It may only include letters, numbers, period (".") and
hyphen ("-") characters.

For a ListedLicenseException, the licenseId will be as specified on the
[SPDX Exceptions List](https://spdx.org/licenses/exceptions-index.html) for the
particular exception.

For a CustomLicenseAddition, the short-form identifier must begin with the
prefix `AdditionRef-` and must be unique within the applicable SPDX namespace.
The short-form identifier may be preceded by an SPDX namespace or a
fully-qualified URI prefix.""" ;
    rdfs:range xsd:string ;
    ns0:term_status "Stable" .

expandedlicensing:additionName a owl:DatatypeProperty ;
    rdfs:comment """An additionName contains the full name of a LicenseAddition, preferably using
the title found in the applicable license addition text or file, or as
otherwise specified by the LicenseAddition's author or steward.

When no such title is specified, using a name from another well-known source or list
of licenses additions (such as OSI or Fedora) is suggested.

If no official or common name is known, any name may be used to aid in
distinguishing the LicenseAddition from other LicenseAdditions.""" ;
    rdfs:range xsd:string ;
    ns0:term_status "Stable" .

expandedlicensing:licenseComment a owl:DatatypeProperty ;
    rdfs:comment """A licenseComment describes general factual information about the License. It
should not contain information (or links to information) that includes any kind
of interpretation about the meaning or effect of the License, even if written
by the license's author.

Examples of information for a licenseComment may include the following:

* If the License's identifier is deprecated, it may briefly explain the reason
  for deprecation.
* It may include the date of release, if identified, for Licenses with multiple
  versions.
* It may include links to other official language translations for the License.
* For LicenseAdditions, it may include a reference to the License(s) with
  which this additional text is typically used.""" ;
    rdfs:range xsd:string ;
    ns0:term_status "Stable" .

expandedlicensing:licenseId a owl:DatatypeProperty ;
    rdfs:comment """A licenseId contains a human-readable, short-form license identifier for a
License. It may only include letters, numbers, period (".") and hyphen ("-")
characters.

For a ListedLicense, the licenseId will be as specified on the
[SPDX License List](https://spdx.org/licenses) for the particular license.

For a CustomLicense, the short-form license identifier must begin with the
prefix `LicenseRef-` and must be unique within the applicable SPDX namespace.
The short-form license ID may be preceded by an SPDX namespace or a
fully-qualified URI prefix.""" ;
    rdfs:range xsd:string ;
    ns0:term_status "Stable" .

expandedlicensing:licenseName a owl:DatatypeProperty ;
    rdfs:comment """A licenseName contains the full name of a License, preferably using the title found
in the applicable license text or file, or as otherwise specified by the
License's author or steward.

When no such title is specified, using a name from another well-known source or list
of licenses (such as OSI or Fedora) is suggested.

If no official or common name is known, any name may be used to aid in
distinguishing the License from other Licenses.""" ;
    rdfs:range xsd:string ;
    ns0:term_status "Stable" .

expandedlicensing:seeAlso a owl:DatatypeProperty ;
    rdfs:comment """A seeAlso defines a cross-reference with a URL where the License or
LicenseAddition can be found in use by one or a few projects.

If applicable, it should include a URL where the license text is posted by
the license steward, particularly if the license steward has made available a
"canonical" primary URL for the license text.

If the license is OSI approved, a seeAlso should be included with the URL for
the license's listing on the OSI website.

The seeAlso URL may refer to a previously-available URL for the License or
LicenseAddition which is no longer active.

Where applicable, the seeAlso URL should include the license text in its
native language. seeAlso URLs to English or other translations may be included
where multiple, equivalent official translations exist.""" ;
    rdfs:range xsd:anyURI ;
    ns0:term_status "Stable" .

security:VexFixedVulnAssessmentRelationship a owl:Class,
        sh:NodeShape ;
    rdfs:comment """VexFixedVulnAssessmentRelationship links a vulnerability to a number of elements
representing VEX products where a vulnerability has been fixed and are no longer
affected. It represents the VEX fixed status.

**Constraints**

When linking elements using a VexFixedVulnAssessmentRelationship, the following
requirements must be observed:

- Elements linked with a VulnVexFixedAssessmentRelationship are constrained to
using the fixedIn relationship type.
- The from: end of the relationship must ve a /Security/Vulnerability classed
element.

**Syntax**

```json
{
  "@type": "VexFixedVulnAssessmentRelationship",
  "@id": "urn:spdx.dev:vex-fixed-in-1",
  "relationshipType": "fixedIn",
  "from": "urn:spdx.dev:vuln-cve-2020-28498",
  "to": ["urn:product-acme-application-1.3"],
  "assessedElement": "urn:npm-elliptic-6.5.4",
  "suppliedBy": ["urn:spdx.dev:agent-jane-doe"],
  "publishedTime": "2021-03-09T11:04:53Z"
}
```""" ;
    rdfs:subClassOf security:VexVulnAssessmentRelationship ;
    ns0:term_status "Stable" .

security:VexUnderInvestigationVulnAssessmentRelationship a owl:Class,
        sh:NodeShape ;
    rdfs:comment """VexUnderInvestigationVulnAssessmentRelationship links a vulnerability to a
number of products stating the vulnerability's impact on them is being
investigated. It represents the VEX under_investigation status.

**Constraints**

When linking elements using a VexUnderInvestigationVulnAssessmentRelationship
the following requirements must be observed:

- Elements linked with a VexUnderInvestigationVulnAssessmentRelationship are
constrained to using the underInvestigationFor relationship type.
- The from: end of the relationship must ve a /Security/Vulnerability classed
element.

**Syntax**

```json
{
  "@type": "VexUnderInvestigationVulnAssessmentRelationship",
  "@id": "urn:spdx.dev:vex-underInvestigation-1",
  "relationshipType": "underInvestigationFor",
  "from": "urn:spdx.dev:vuln-cve-2020-28498",
  "to": ["urn:product-acme-application-1.3"],
  "assessedElement": "urn:npm-elliptic-6.5.2",
  "suppliedBy": ["urn:spdx.dev:agent-jane-doe"],
  "publishedTime": "2021-03-09T11:04:53Z"
}
```""" ;
    rdfs:subClassOf security:VexVulnAssessmentRelationship ;
    ns0:term_status "Stable" .

<https://spdx.org/rdf/v3/AI/SafetyRiskAssessmentType/high> a owl:NamedIndividual,
        ai:SafetyRiskAssessmentType .

<https://spdx.org/rdf/v3/AI/SafetyRiskAssessmentType/low> a owl:NamedIndividual,
        ai:SafetyRiskAssessmentType .

<https://spdx.org/rdf/v3/AI/SafetyRiskAssessmentType/medium> a owl:NamedIndividual,
        ai:SafetyRiskAssessmentType .

<https://spdx.org/rdf/v3/AI/SafetyRiskAssessmentType/serious> a owl:NamedIndividual,
        ai:SafetyRiskAssessmentType .

ai:autonomyType a owl:ObjectProperty ;
    rdfs:comment """AutonomyType indicates if a human is involved in any of the decisions of the AI software
or if that software is fully automatic.""" ;
    rdfs:domain ai:AIPackage ;
    rdfs:range core:PresenceType ;
    ns0:term_status "Stable" .

ai:domain a owl:DatatypeProperty ;
    rdfs:comment """Domain describes the domain in which the AI model contained in the AI software
can be expected to operate successfully. Examples include computer vision, natural language etc.""" ;
    rdfs:domain ai:AIPackage ;
    rdfs:range xsd:string ;
    ns0:term_status "Stable" .

ai:energyConsumption a owl:DatatypeProperty ;
    rdfs:comment """EnergyConsumption captures the amount of energy needed to train and operate the AI model. 
This value is also known as training energy consumption or inference energy consumption.""" ;
    rdfs:domain ai:AIPackage ;
    rdfs:range xsd:string ;
    ns0:term_status "Stable" .

ai:hyperparameter a owl:ObjectProperty ;
    rdfs:comment """This field records a hyperparameter value.
Hyperparameters are parameters of the machine learning model that are used to control the learning process,
for example the optimization and learning rate used during the training of the model.""" ;
    rdfs:domain ai:AIPackage ;
    rdfs:range core:DictionaryEntry ;
    ns0:term_status "Stable" .

ai:informationAboutApplication a owl:DatatypeProperty ;
    rdfs:comment """InformationAboutApplication describes any relevant information in free form text about 
how the AI model is used inside the software, as well as any relevant pre-processing steps, third party APIs etc.""" ;
    rdfs:domain ai:AIPackage ;
    rdfs:range xsd:string ;
    ns0:term_status "Stable" .

ai:informationAboutTraining a owl:DatatypeProperty ;
    rdfs:comment """InformationAboutTraining describes the specific steps involved in the training of the AI model.
For example, it can be specified whether supervised fine-tuning 
or active learning is used as part of training the model.""" ;
    rdfs:domain ai:AIPackage ;
    rdfs:range xsd:string ;
    ns0:term_status "Stable" .

ai:limitation a owl:DatatypeProperty ;
    rdfs:comment """Limitation captures a limitation of the AI Package (or of the AI models present in the AI package),
expressed as free form text. Note that this is not guaranteed to be exhaustive.
For instance, a limitation might be that the AI package cannot be used on datasets from a certain demography.""" ;
    rdfs:domain ai:AIPackage ;
    rdfs:range xsd:string ;
    ns0:term_status "Stable" .

ai:metric a owl:ObjectProperty ;
    rdfs:comment """Metric records the measurement with which the AI model was evaluated. 
This makes statements about the prediction quality including uncertainty,
accuracy, characteristics of the tested population, quality, fairness, explainability, robustness etc.""" ;
    rdfs:domain ai:AIPackage ;
    rdfs:range core:DictionaryEntry ;
    ns0:term_status "Stable" .

ai:metricDecisionThreshold a owl:ObjectProperty ;
    rdfs:comment """Each metric might be computed based on a decision threshold. 
For instance, precision or recall is typically computed by checking
if the probability of the outcome is larger than 0.5.
Each decision threshold should match with a metric field defined in the AI Package.""" ;
    rdfs:domain ai:AIPackage ;
    rdfs:range core:DictionaryEntry ;
    ns0:term_status "Stable" .

ai:modelDataPreprocessing a owl:DatatypeProperty ;
    rdfs:comment """ModelDataPreprocessing is a free form text that describes the preprocessing steps
applied to the training data before training of the model(s) contained in the AI software.""" ;
    rdfs:domain ai:AIPackage ;
    rdfs:range xsd:string ;
    ns0:term_status "Stable" .

ai:modelExplainability a owl:DatatypeProperty ;
    rdfs:comment """ModelExplainability is a free form text that lists the different explainability mechanisms
(such as SHAP, or other model specific explainability mechanisms) that can be used to explain the model.""" ;
    rdfs:domain ai:AIPackage ;
    rdfs:range xsd:string ;
    ns0:term_status "Stable" .

ai:safetyRiskAssessment a owl:ObjectProperty ;
    rdfs:comment """SafetyRiskAssessment categorizes the safety risk impact of the AI software
in accordance with Article 20 of [EC Regulation No 765/2008](https://ec.europa.eu/docsroom/documents/17107/attachments/1/translations/en/renditions/pdf).""" ;
    rdfs:domain ai:AIPackage ;
    rdfs:range ai:SafetyRiskAssessmentType ;
    ns0:term_status "Stable" .

ai:sensitivePersonalInformation a owl:ObjectProperty ;
    rdfs:comment """SensitivePersonalInformation notes if sensitive personal information
is used in the training or inference of the AI models.
This might include biometric data, addresses or other data that can be used to infer a person's identity.""" ;
    rdfs:domain ai:AIPackage ;
    rdfs:range core:PresenceType ;
    ns0:term_status "Stable" .

ai:standardCompliance a owl:DatatypeProperty ;
    rdfs:comment """StandardCompliance captures a standard that the AI software complies with. 
This includes both published and unpublished standards, for example ISO, IEEE, ETSI etc. 
The standard could (but not necessarily have to) be used to satisfy a legal or regulatory requirement.""" ;
    rdfs:domain ai:AIPackage ;
    rdfs:range xsd:string ;
    ns0:term_status "Stable" .

ai:typeOfModel a owl:DatatypeProperty ;
    rdfs:comment """TypeOfModel records the type of the AI model(s) used in the software. 
For instance, if it is a supervised model, unsupervised model, reinforcement learning model or a combination of those.""" ;
    rdfs:domain ai:AIPackage ;
    rdfs:range xsd:string ;
    ns0:term_status "Stable" .

build:buildEndTime a owl:DatatypeProperty ;
    rdfs:comment "buildEndTime describes the time at which a build stops or finishes. This value is typically recorded by the builder." ;
    rdfs:domain build:Build ;
    rdfs:range core:DateTime ;
    ns0:term_status "Stable" .

build:buildId a owl:DatatypeProperty ;
    rdfs:comment "A buildId is a locally unique identifier to identify a unique instance of a build. This identifier differs based on build toolchain, platform, or naming convention used by an organization or standard." ;
    rdfs:domain build:Build ;
    rdfs:range xsd:string ;
    ns0:term_status "Stable" .

build:buildStartTime a owl:DatatypeProperty ;
    rdfs:comment "buildStartTime is the time at which a build is triggered. The builder typically records this value." ;
    rdfs:domain build:Build ;
    rdfs:range core:DateTime ;
    ns0:term_status "Stable" .

build:buildType a owl:DatatypeProperty ;
    rdfs:comment "A buildType is a URI expressing the toolchain, platform, or infrastructure that the build was invoked on. For example, if the build was invoked on GitHub's CI platform using github actions, the buildType can be expressed as `https://github.com/actions`. In contrast, if the build was invoked on a local machine, the buildType can be expressed as `file://username@host/path/to/build`." ;
    rdfs:domain build:Build ;
    rdfs:range xsd:anyURI ;
    ns0:term_status "Stable" .

build:configSourceDigest a owl:ObjectProperty ;
    rdfs:comment "configSourceDigest is the checksum of the build configuration file used by a builder to execute a build. This Property uses the Core model's [Hash](../../Core/Classes/Hash.md) class." ;
    rdfs:domain build:Build ;
    rdfs:range core:Hash ;
    ns0:term_status "Stable" .

build:configSourceEntrypoint a owl:DatatypeProperty ;
    rdfs:comment """A build entrypoint is the invoked executable of a build which always runs when the build is triggered. For example, when a build is triggered by running a shell script, the entrypoint is `script.sh`. In terms of a declared build, the entrypoint is the position in a configuration file or a build declaration which is always run when the build is triggered. For example, in the following configuration file, the entrypoint of the build is `publish`.

```
name: Publish packages to PyPI

on:
create:
tags: "*"

jobs:
publish:
runs-on: ubuntu-latest
if: startsWith(github.ref, 'refs/tags/')
steps:

...
```""" ;
    rdfs:domain build:Build ;
    rdfs:range xsd:string ;
    ns0:term_status "Stable" .

build:configSourceUri a owl:DatatypeProperty ;
    rdfs:comment """If a build configuration exists for the toolchain or platform performing the build, the configSourceUri of a build is the URI of that build configuration. For example, a build triggered by a GitHub action is defined by a build configuration YAML file. In this case, the configSourceUri is the URL of that YAML file. 
m""" ;
    rdfs:domain build:Build ;
    rdfs:range xsd:anyURI ;
    ns0:term_status "Stable" .

build:environment a owl:ObjectProperty ;
    rdfs:comment "environment is a map of environment variables and values that are set during a build session. This is different from the [parameters](parameters.md) property in that it describes the environment variables set before a build is invoked rather than the variables provided to the builder." ;
    rdfs:domain build:Build ;
    rdfs:range core:DictionaryEntry ;
    ns0:term_status "Stable" .

build:parameters a owl:ObjectProperty ;
    rdfs:comment "parameters is a key-value map of all build parameters and their values that were provided to the builder for a build instance. This is different from the [environment](environment.md) property in that the keys and values are provided as command line arguments or a configuration file to the builder." ;
    rdfs:domain build:Build ;
    rdfs:range core:DictionaryEntry ;
    ns0:term_status "Stable" .

<https://spdx.org/rdf/v3/Core/AnnotationType/other> a owl:NamedIndividual,
        core:AnnotationType .

<https://spdx.org/rdf/v3/Core/AnnotationType/review> a owl:NamedIndividual,
        core:AnnotationType .

core:Bom a owl:Class,
        sh:NodeShape ;
    rdfs:comment """A Bill Of Materials (BOM) is a container for a grouping of SPDX-3.0 content
characterizing details about a product.
This could include details of the content and composition of the product,
provenence details of the product and/or
its composition, licensing information, known quality or security issues, etc.""" ;
    rdfs:subClassOf core:Bundle ;
    ns0:term_status "Stable" .

<https://spdx.org/rdf/v3/Core/ExternalIdentifierType/cpe22> a owl:NamedIndividual,
        core:ExternalIdentifierType .

<https://spdx.org/rdf/v3/Core/ExternalIdentifierType/cpe23> a owl:NamedIndividual,
        core:ExternalIdentifierType .

<https://spdx.org/rdf/v3/Core/ExternalIdentifierType/cve> a owl:NamedIndividual,
        core:ExternalIdentifierType .

<https://spdx.org/rdf/v3/Core/ExternalIdentifierType/email> a owl:NamedIndividual,
        core:ExternalIdentifierType .

<https://spdx.org/rdf/v3/Core/ExternalIdentifierType/gitoid> a owl:NamedIndividual,
        core:ExternalIdentifierType .

<https://spdx.org/rdf/v3/Core/ExternalIdentifierType/other> a owl:NamedIndividual,
        core:ExternalIdentifierType .

<https://spdx.org/rdf/v3/Core/ExternalIdentifierType/pkgUrl> a owl:NamedIndividual,
        core:ExternalIdentifierType .

<https://spdx.org/rdf/v3/Core/ExternalIdentifierType/securityOther> a owl:NamedIndividual,
        core:ExternalIdentifierType .

<https://spdx.org/rdf/v3/Core/ExternalIdentifierType/swhid> a owl:NamedIndividual,
        core:ExternalIdentifierType .

<https://spdx.org/rdf/v3/Core/ExternalIdentifierType/swid> a owl:NamedIndividual,
        core:ExternalIdentifierType .

<https://spdx.org/rdf/v3/Core/ExternalIdentifierType/urlScheme> a owl:NamedIndividual,
        core:ExternalIdentifierType .

<https://spdx.org/rdf/v3/Core/ExternalRefType/altDownloadLocation> a owl:NamedIndividual,
        core:ExternalRefType .

<https://spdx.org/rdf/v3/Core/ExternalRefType/altWebPage> a owl:NamedIndividual,
        core:ExternalRefType .

<https://spdx.org/rdf/v3/Core/ExternalRefType/binaryArtifact> a owl:NamedIndividual,
        core:ExternalRefType .

<https://spdx.org/rdf/v3/Core/ExternalRefType/bower> a owl:NamedIndividual,
        core:ExternalRefType .

<https://spdx.org/rdf/v3/Core/ExternalRefType/buildMeta> a owl:NamedIndividual,
        core:ExternalRefType .

<https://spdx.org/rdf/v3/Core/ExternalRefType/buildSystem> a owl:NamedIndividual,
        core:ExternalRefType .

<https://spdx.org/rdf/v3/Core/ExternalRefType/certificationReport> a owl:NamedIndividual,
        core:ExternalRefType .

<https://spdx.org/rdf/v3/Core/ExternalRefType/chat> a owl:NamedIndividual,
        core:ExternalRefType .

<https://spdx.org/rdf/v3/Core/ExternalRefType/componentAnalysisReport> a owl:NamedIndividual,
        core:ExternalRefType .

<https://spdx.org/rdf/v3/Core/ExternalRefType/documentation> a owl:NamedIndividual,
        core:ExternalRefType .

<https://spdx.org/rdf/v3/Core/ExternalRefType/dynamicAnalysisReport> a owl:NamedIndividual,
        core:ExternalRefType .

<https://spdx.org/rdf/v3/Core/ExternalRefType/eolNotice> a owl:NamedIndividual,
        core:ExternalRefType .

<https://spdx.org/rdf/v3/Core/ExternalRefType/exportControlAssessment> a owl:NamedIndividual,
        core:ExternalRefType .

<https://spdx.org/rdf/v3/Core/ExternalRefType/funding> a owl:NamedIndividual,
        core:ExternalRefType .

<https://spdx.org/rdf/v3/Core/ExternalRefType/issueTracker> a owl:NamedIndividual,
        core:ExternalRefType .

<https://spdx.org/rdf/v3/Core/ExternalRefType/license> a owl:NamedIndividual,
        core:ExternalRefType .

<https://spdx.org/rdf/v3/Core/ExternalRefType/mailingList> a owl:NamedIndividual,
        core:ExternalRefType .

<https://spdx.org/rdf/v3/Core/ExternalRefType/mavenCentral> a owl:NamedIndividual,
        core:ExternalRefType .

<https://spdx.org/rdf/v3/Core/ExternalRefType/metrics> a owl:NamedIndividual,
        core:ExternalRefType .

<https://spdx.org/rdf/v3/Core/ExternalRefType/npm> a owl:NamedIndividual,
        core:ExternalRefType .

<https://spdx.org/rdf/v3/Core/ExternalRefType/nuget> a owl:NamedIndividual,
        core:ExternalRefType .

<https://spdx.org/rdf/v3/Core/ExternalRefType/other> a owl:NamedIndividual,
        core:ExternalRefType .

<https://spdx.org/rdf/v3/Core/ExternalRefType/privacyAssessment> a owl:NamedIndividual,
        core:ExternalRefType .

<https://spdx.org/rdf/v3/Core/ExternalRefType/productMetadata> a owl:NamedIndividual,
        core:ExternalRefType .

<https://spdx.org/rdf/v3/Core/ExternalRefType/purchaseOrder> a owl:NamedIndividual,
        core:ExternalRefType .

<https://spdx.org/rdf/v3/Core/ExternalRefType/qualityAssessmentReport> a owl:NamedIndividual,
        core:ExternalRefType .

<https://spdx.org/rdf/v3/Core/ExternalRefType/releaseHistory> a owl:NamedIndividual,
        core:ExternalRefType .

<https://spdx.org/rdf/v3/Core/ExternalRefType/releaseNotes> a owl:NamedIndividual,
        core:ExternalRefType .

<https://spdx.org/rdf/v3/Core/ExternalRefType/riskAssessment> a owl:NamedIndividual,
        core:ExternalRefType .

<https://spdx.org/rdf/v3/Core/ExternalRefType/runtimeAnalysisReport> a owl:NamedIndividual,
        core:ExternalRefType .

<https://spdx.org/rdf/v3/Core/ExternalRefType/secureSoftwareAttestation> a owl:NamedIndividual,
        core:ExternalRefType .

<https://spdx.org/rdf/v3/Core/ExternalRefType/securityAdversaryModel> a owl:NamedIndividual,
        core:ExternalRefType .

<https://spdx.org/rdf/v3/Core/ExternalRefType/securityAdvisory> a owl:NamedIndividual,
        core:ExternalRefType .

<https://spdx.org/rdf/v3/Core/ExternalRefType/securityFix> a owl:NamedIndividual,
        core:ExternalRefType .

<https://spdx.org/rdf/v3/Core/ExternalRefType/securityOther> a owl:NamedIndividual,
        core:ExternalRefType .

<https://spdx.org/rdf/v3/Core/ExternalRefType/securityPenTestReport> a owl:NamedIndividual,
        core:ExternalRefType .

<https://spdx.org/rdf/v3/Core/ExternalRefType/securityPolicy> a owl:NamedIndividual,
        core:ExternalRefType .

<https://spdx.org/rdf/v3/Core/ExternalRefType/securityThreatModel> a owl:NamedIndividual,
        core:ExternalRefType .

<https://spdx.org/rdf/v3/Core/ExternalRefType/socialMedia> a owl:NamedIndividual,
        core:ExternalRefType .

<https://spdx.org/rdf/v3/Core/ExternalRefType/sourceArtifact> a owl:NamedIndividual,
        core:ExternalRefType .

<https://spdx.org/rdf/v3/Core/ExternalRefType/staticAnalysisReport> a owl:NamedIndividual,
        core:ExternalRefType .

<https://spdx.org/rdf/v3/Core/ExternalRefType/support> a owl:NamedIndividual,
        core:ExternalRefType .

<https://spdx.org/rdf/v3/Core/ExternalRefType/vcs> a owl:NamedIndividual,
        core:ExternalRefType .

<https://spdx.org/rdf/v3/Core/ExternalRefType/vulnerabilityDisclosureReport> a owl:NamedIndividual,
        core:ExternalRefType .

<https://spdx.org/rdf/v3/Core/ExternalRefType/vulnerabilityExploitabilityAssessment> a owl:NamedIndividual,
        core:ExternalRefType .

<https://spdx.org/rdf/v3/Core/HashAlgorithm/blake2b256> a owl:NamedIndividual,
        core:HashAlgorithm .

<https://spdx.org/rdf/v3/Core/HashAlgorithm/blake2b384> a owl:NamedIndividual,
        core:HashAlgorithm .

<https://spdx.org/rdf/v3/Core/HashAlgorithm/blake2b512> a owl:NamedIndividual,
        core:HashAlgorithm .

<https://spdx.org/rdf/v3/Core/HashAlgorithm/blake3> a owl:NamedIndividual,
        core:HashAlgorithm .

<https://spdx.org/rdf/v3/Core/HashAlgorithm/crystalsDilithium> a owl:NamedIndividual,
        core:HashAlgorithm .

<https://spdx.org/rdf/v3/Core/HashAlgorithm/crystalsKyber> a owl:NamedIndividual,
        core:HashAlgorithm .

<https://spdx.org/rdf/v3/Core/HashAlgorithm/falcon> a owl:NamedIndividual,
        core:HashAlgorithm .

<https://spdx.org/rdf/v3/Core/HashAlgorithm/md2> a owl:NamedIndividual,
        core:HashAlgorithm .

<https://spdx.org/rdf/v3/Core/HashAlgorithm/md4> a owl:NamedIndividual,
        core:HashAlgorithm .

<https://spdx.org/rdf/v3/Core/HashAlgorithm/md5> a owl:NamedIndividual,
        core:HashAlgorithm .

<https://spdx.org/rdf/v3/Core/HashAlgorithm/md6> a owl:NamedIndividual,
        core:HashAlgorithm .

<https://spdx.org/rdf/v3/Core/HashAlgorithm/other> a owl:NamedIndividual,
        core:HashAlgorithm .

<https://spdx.org/rdf/v3/Core/HashAlgorithm/sha1> a owl:NamedIndividual,
        core:HashAlgorithm .

<https://spdx.org/rdf/v3/Core/HashAlgorithm/sha224> a owl:NamedIndividual,
        core:HashAlgorithm .

<https://spdx.org/rdf/v3/Core/HashAlgorithm/sha256> a owl:NamedIndividual,
        core:HashAlgorithm .

<https://spdx.org/rdf/v3/Core/HashAlgorithm/sha384> a owl:NamedIndividual,
        core:HashAlgorithm .

<https://spdx.org/rdf/v3/Core/HashAlgorithm/sha3_224> a owl:NamedIndividual,
        core:HashAlgorithm .

<https://spdx.org/rdf/v3/Core/HashAlgorithm/sha3_256> a owl:NamedIndividual,
        core:HashAlgorithm .

<https://spdx.org/rdf/v3/Core/HashAlgorithm/sha3_384> a owl:NamedIndividual,
        core:HashAlgorithm .

<https://spdx.org/rdf/v3/Core/HashAlgorithm/sha3_512> a owl:NamedIndividual,
        core:HashAlgorithm .

<https://spdx.org/rdf/v3/Core/HashAlgorithm/sha512> a owl:NamedIndividual,
        core:HashAlgorithm .

<https://spdx.org/rdf/v3/Core/HashAlgorithm/spdxPvcSha1> a owl:NamedIndividual,
        core:HashAlgorithm .

<https://spdx.org/rdf/v3/Core/HashAlgorithm/spdxPvcSha256> a owl:NamedIndividual,
        core:HashAlgorithm .

<https://spdx.org/rdf/v3/Core/HashAlgorithm/sphincsPlus> a owl:NamedIndividual,
        core:HashAlgorithm .

<https://spdx.org/rdf/v3/Core/LifecycleScopeType/build> a owl:NamedIndividual,
        core:LifecycleScopeType .

<https://spdx.org/rdf/v3/Core/LifecycleScopeType/design> a owl:NamedIndividual,
        core:LifecycleScopeType .

<https://spdx.org/rdf/v3/Core/LifecycleScopeType/development> a owl:NamedIndividual,
        core:LifecycleScopeType .

<https://spdx.org/rdf/v3/Core/LifecycleScopeType/other> a owl:NamedIndividual,
        core:LifecycleScopeType .

<https://spdx.org/rdf/v3/Core/LifecycleScopeType/runtime> a owl:NamedIndividual,
        core:LifecycleScopeType .

<https://spdx.org/rdf/v3/Core/LifecycleScopeType/test> a owl:NamedIndividual,
        core:LifecycleScopeType .

<https://spdx.org/rdf/v3/Core/PresenceType/no> a owl:NamedIndividual,
        core:PresenceType .

<https://spdx.org/rdf/v3/Core/PresenceType/noAssertion> a owl:NamedIndividual,
        core:PresenceType .

<https://spdx.org/rdf/v3/Core/PresenceType/yes> a owl:NamedIndividual,
        core:PresenceType .

<https://spdx.org/rdf/v3/Core/ProfileIdentifierType/ai> a owl:NamedIndividual,
        core:ProfileIdentifierType .

<https://spdx.org/rdf/v3/Core/ProfileIdentifierType/build> a owl:NamedIndividual,
        core:ProfileIdentifierType .

<https://spdx.org/rdf/v3/Core/ProfileIdentifierType/core> a owl:NamedIndividual,
        core:ProfileIdentifierType .

<https://spdx.org/rdf/v3/Core/ProfileIdentifierType/dataset> a owl:NamedIndividual,
        core:ProfileIdentifierType .

<https://spdx.org/rdf/v3/Core/ProfileIdentifierType/expandedLicensing> a owl:NamedIndividual,
        core:ProfileIdentifierType .

<https://spdx.org/rdf/v3/Core/ProfileIdentifierType/extension> a owl:NamedIndividual,
        core:ProfileIdentifierType .

<https://spdx.org/rdf/v3/Core/ProfileIdentifierType/security> a owl:NamedIndividual,
        core:ProfileIdentifierType .

<https://spdx.org/rdf/v3/Core/ProfileIdentifierType/simpleLicensing> a owl:NamedIndividual,
        core:ProfileIdentifierType .

<https://spdx.org/rdf/v3/Core/ProfileIdentifierType/software> a owl:NamedIndividual,
        core:ProfileIdentifierType .

<https://spdx.org/rdf/v3/Core/ProfileIdentifierType/usage> a owl:NamedIndividual,
        core:ProfileIdentifierType .

<https://spdx.org/rdf/v3/Core/RelationshipCompleteness/complete> a owl:NamedIndividual,
        core:RelationshipCompleteness .

<https://spdx.org/rdf/v3/Core/RelationshipCompleteness/incomplete> a owl:NamedIndividual,
        core:RelationshipCompleteness .

<https://spdx.org/rdf/v3/Core/RelationshipCompleteness/noAssertion> a owl:NamedIndividual,
        core:RelationshipCompleteness .

<https://spdx.org/rdf/v3/Core/RelationshipType/affects> a owl:NamedIndividual,
        core:RelationshipType .

<https://spdx.org/rdf/v3/Core/RelationshipType/amendedBy> a owl:NamedIndividual,
        core:RelationshipType .

<https://spdx.org/rdf/v3/Core/RelationshipType/ancestorOf> a owl:NamedIndividual,
        core:RelationshipType .

<https://spdx.org/rdf/v3/Core/RelationshipType/availableFrom> a owl:NamedIndividual,
        core:RelationshipType .

<https://spdx.org/rdf/v3/Core/RelationshipType/configures> a owl:NamedIndividual,
        core:RelationshipType .

<https://spdx.org/rdf/v3/Core/RelationshipType/contains> a owl:NamedIndividual,
        core:RelationshipType .

<https://spdx.org/rdf/v3/Core/RelationshipType/coordinatedBy> a owl:NamedIndividual,
        core:RelationshipType .

<https://spdx.org/rdf/v3/Core/RelationshipType/copiedTo> a owl:NamedIndividual,
        core:RelationshipType .

<https://spdx.org/rdf/v3/Core/RelationshipType/delegatedTo> a owl:NamedIndividual,
        core:RelationshipType .

<https://spdx.org/rdf/v3/Core/RelationshipType/dependsOn> a owl:NamedIndividual,
        core:RelationshipType .

<https://spdx.org/rdf/v3/Core/RelationshipType/descendantOf> a owl:NamedIndividual,
        core:RelationshipType .

<https://spdx.org/rdf/v3/Core/RelationshipType/describes> a owl:NamedIndividual,
        core:RelationshipType .

<https://spdx.org/rdf/v3/Core/RelationshipType/doesNotAffect> a owl:NamedIndividual,
        core:RelationshipType .

<https://spdx.org/rdf/v3/Core/RelationshipType/expandsTo> a owl:NamedIndividual,
        core:RelationshipType .

<https://spdx.org/rdf/v3/Core/RelationshipType/exploitCreatedBy> a owl:NamedIndividual,
        core:RelationshipType .

<https://spdx.org/rdf/v3/Core/RelationshipType/fixedBy> a owl:NamedIndividual,
        core:RelationshipType .

<https://spdx.org/rdf/v3/Core/RelationshipType/fixedIn> a owl:NamedIndividual,
        core:RelationshipType .

<https://spdx.org/rdf/v3/Core/RelationshipType/foundBy> a owl:NamedIndividual,
        core:RelationshipType .

<https://spdx.org/rdf/v3/Core/RelationshipType/generates> a owl:NamedIndividual,
        core:RelationshipType .

<https://spdx.org/rdf/v3/Core/RelationshipType/hasAddedFile> a owl:NamedIndividual,
        core:RelationshipType .

<https://spdx.org/rdf/v3/Core/RelationshipType/hasAssessmentFor> a owl:NamedIndividual,
        core:RelationshipType .

<https://spdx.org/rdf/v3/Core/RelationshipType/hasAssociatedVulnerability> a owl:NamedIndividual,
        core:RelationshipType .

<https://spdx.org/rdf/v3/Core/RelationshipType/hasConcludedLicense> a owl:NamedIndividual,
        core:RelationshipType .

<https://spdx.org/rdf/v3/Core/RelationshipType/hasDataFile> a owl:NamedIndividual,
        core:RelationshipType .

<https://spdx.org/rdf/v3/Core/RelationshipType/hasDeclaredLicense> a owl:NamedIndividual,
        core:RelationshipType .

<https://spdx.org/rdf/v3/Core/RelationshipType/hasDeletedFile> a owl:NamedIndividual,
        core:RelationshipType .

<https://spdx.org/rdf/v3/Core/RelationshipType/hasDependencyManifest> a owl:NamedIndividual,
        core:RelationshipType .

<https://spdx.org/rdf/v3/Core/RelationshipType/hasDistributionArtifact> a owl:NamedIndividual,
        core:RelationshipType .

<https://spdx.org/rdf/v3/Core/RelationshipType/hasDocumentation> a owl:NamedIndividual,
        core:RelationshipType .

<https://spdx.org/rdf/v3/Core/RelationshipType/hasDynamicLink> a owl:NamedIndividual,
        core:RelationshipType .

<https://spdx.org/rdf/v3/Core/RelationshipType/hasEvidence> a owl:NamedIndividual,
        core:RelationshipType .

<https://spdx.org/rdf/v3/Core/RelationshipType/hasExample> a owl:NamedIndividual,
        core:RelationshipType .

<https://spdx.org/rdf/v3/Core/RelationshipType/hasHost> a owl:NamedIndividual,
        core:RelationshipType .

<https://spdx.org/rdf/v3/Core/RelationshipType/hasInputs> a owl:NamedIndividual,
        core:RelationshipType .

<https://spdx.org/rdf/v3/Core/RelationshipType/hasMetadata> a owl:NamedIndividual,
        core:RelationshipType .

<https://spdx.org/rdf/v3/Core/RelationshipType/hasOptionalComponent> a owl:NamedIndividual,
        core:RelationshipType .

<https://spdx.org/rdf/v3/Core/RelationshipType/hasOptionalDependency> a owl:NamedIndividual,
        core:RelationshipType .

<https://spdx.org/rdf/v3/Core/RelationshipType/hasOutputs> a owl:NamedIndividual,
        core:RelationshipType .

<https://spdx.org/rdf/v3/Core/RelationshipType/hasPrerequsite> a owl:NamedIndividual,
        core:RelationshipType .

<https://spdx.org/rdf/v3/Core/RelationshipType/hasProvidedDependency> a owl:NamedIndividual,
        core:RelationshipType .

<https://spdx.org/rdf/v3/Core/RelationshipType/hasRequirement> a owl:NamedIndividual,
        core:RelationshipType .

<https://spdx.org/rdf/v3/Core/RelationshipType/hasSpecification> a owl:NamedIndividual,
        core:RelationshipType .

<https://spdx.org/rdf/v3/Core/RelationshipType/hasStaticLink> a owl:NamedIndividual,
        core:RelationshipType .

<https://spdx.org/rdf/v3/Core/RelationshipType/hasTest> a owl:NamedIndividual,
        core:RelationshipType .

<https://spdx.org/rdf/v3/Core/RelationshipType/hasTestCase> a owl:NamedIndividual,
        core:RelationshipType .

<https://spdx.org/rdf/v3/Core/RelationshipType/hasVariant> a owl:NamedIndividual,
        core:RelationshipType .

<https://spdx.org/rdf/v3/Core/RelationshipType/invokedBy> a owl:NamedIndividual,
        core:RelationshipType .

<https://spdx.org/rdf/v3/Core/RelationshipType/modifiedBy> a owl:NamedIndividual,
        core:RelationshipType .

<https://spdx.org/rdf/v3/Core/RelationshipType/other> a owl:NamedIndividual,
        core:RelationshipType .

<https://spdx.org/rdf/v3/Core/RelationshipType/packagedBy> a owl:NamedIndividual,
        core:RelationshipType .

<https://spdx.org/rdf/v3/Core/RelationshipType/patchedBy> a owl:NamedIndividual,
        core:RelationshipType .

<https://spdx.org/rdf/v3/Core/RelationshipType/publishedBy> a owl:NamedIndividual,
        core:RelationshipType .

<https://spdx.org/rdf/v3/Core/RelationshipType/reportedBy> a owl:NamedIndividual,
        core:RelationshipType .

<https://spdx.org/rdf/v3/Core/RelationshipType/republishedBy> a owl:NamedIndividual,
        core:RelationshipType .

<https://spdx.org/rdf/v3/Core/RelationshipType/serializedInArtifact> a owl:NamedIndividual,
        core:RelationshipType .

<https://spdx.org/rdf/v3/Core/RelationshipType/testedOn> a owl:NamedIndividual,
        core:RelationshipType .

<https://spdx.org/rdf/v3/Core/RelationshipType/trainedOn> a owl:NamedIndividual,
        core:RelationshipType .

<https://spdx.org/rdf/v3/Core/RelationshipType/underInvestigationFor> a owl:NamedIndividual,
        core:RelationshipType .

<https://spdx.org/rdf/v3/Core/RelationshipType/usesTool> a owl:NamedIndividual,
        core:RelationshipType .

core:algorithm a owl:ObjectProperty ;
    rdfs:comment "An algorithm specifies the algorithm that was used for calculating the hash value." ;
    rdfs:domain core:Hash ;
    rdfs:range core:HashAlgorithm ;
    ns0:term_status "Stable" .

core:annotationType a owl:ObjectProperty ;
    rdfs:comment "An annotationType describes the type of an annotation." ;
    rdfs:domain core:Annotation ;
    rdfs:range core:AnnotationType ;
    ns0:term_status "Stable" .

core:begin a owl:DatatypeProperty ;
    rdfs:comment "begin is a positive integer that defines the beginning of a range." ;
    rdfs:domain core:PositiveIntegerRange ;
    rdfs:range xsd:positiveInteger ;
    ns0:term_status "Stable" .

core:builtTime a owl:DatatypeProperty ;
    rdfs:comment "A builtTime specifies the time an artifact was built." ;
    rdfs:domain core:Artifact ;
    rdfs:range core:DateTime ;
    ns0:term_status "Stable" .

core:completeness a owl:ObjectProperty ;
    rdfs:comment """Completeness gives information about whether the provided relationships are
complete, known to be incomplete or if no assertion is made either way.""" ;
    rdfs:domain core:Relationship ;
    rdfs:range core:RelationshipCompleteness ;
    ns0:term_status "Stable" .

core:context a owl:DatatypeProperty ;
    rdfs:comment """A context gives information about the circumstances or unifying properties
that Elements of the bundle have been assembled under.""" ;
    rdfs:domain core:Bundle ;
    rdfs:range xsd:string ;
    ns0:term_status "Stable" .

core:created a owl:DatatypeProperty ;
    rdfs:comment """Created is a date that identifies when the Element was originally created.
The time stamp can serve as an indication as to whether the analysis needs to be updated. This is often the date of last change (e.g., a git commit date), not the date when the SPDX data was created, as doing so supports reproducible builds.""" ;
    rdfs:domain core:CreationInfo ;
    rdfs:range core:DateTime ;
    ns0:term_status "Stable" .

core:createdBy a owl:ObjectProperty ;
    rdfs:comment """CreatedBy identifies who or what created the Element.
The generation method will assist the recipient of the Element in assessing
the general reliability/accuracy of the analysis information.""" ;
    rdfs:domain core:CreationInfo ;
    rdfs:range core:Agent ;
    ns0:term_status "Stable" .

core:createdUsing a owl:ObjectProperty ;
    rdfs:comment """CreatedUsing identifies the tooling that was used during the creation of the Element.
The generation method will assist the recipient of the Element in assessing
the general reliability/accuracy of the analysis information.""" ;
    rdfs:domain core:CreationInfo ;
    rdfs:range core:Tool ;
    ns0:term_status "Stable" .

core:creationInfo a owl:ObjectProperty ;
    rdfs:comment "CreationInfo provides information about the creation of the Element." ;
    rdfs:domain core:Element ;
    rdfs:range core:CreationInfo ;
    ns0:term_status "Stable" .

core:dataLicense a owl:DatatypeProperty ;
    rdfs:comment """The data license provides the license under which the SPDX documentation of the Element can be used.
This is to alleviate any concern that content (the data or database) in an SPDX file
is subject to any form of intellectual property right that could restrict the re-use
of the information or the creation of another SPDX file for the same project(s).
This approach avoids intellectual property and related restrictions over the SPDX file,
however individuals can still contract with each other to restrict release
of specific collections of SPDX files (which map to software bill of materials)
and the identification of the supplier of SPDX files.
Compliance with this document includes populating the SPDX fields therein
with data related to such fields ("SPDX-Metadata"). 
This document contains numerous fields where an SPDX file creator may provide
relevant explanatory text in SPDX-Metadata. Without opining on the lawfulness
of "database rights" (in jurisdictions where applicable),
such explanatory text is copyrightable subject matter in most Berne Convention countries.
By using the SPDX specification, or any portion hereof,
you hereby agree that any copyright rights (as determined by your jurisdiction)
in any SPDX-Metadata, including without limitation explanatory text,
shall be subject to the terms of the Creative Commons CC0 1.0 Universal license. 
For SPDX-Metadata not containing any copyright rights, 
you hereby agree and acknowledge that the SPDX-Metadata is provided to you "as-is"
and without any representations or warranties of any kind concerning the SPDX-Metadata,
express, implied, statutory or otherwise, including without limitation warranties
of title, merchantability, fitness for a particular purpose, non-infringement,
or the absence of latent or other defects, accuracy, or the presence or absence of errors,
whether or not discoverable, all to the greatest extent permissible under applicable law.""" ;
    rdfs:domain core:CreationInfo ;
    rdfs:range xsd:string ;
    ns0:term_status "Stable" .

core:definingDocument a owl:ObjectProperty ;
    rdfs:comment "A definingDocument property is used to link the Element identifier for an Element defined external to a given SpdxDocument to an Artifact Element representing the SPDX serialization instance which contains the definition for the Element." ;
    rdfs:domain core:ExternalMap ;
    rdfs:range core:Artifact ;
    ns0:term_status "Stable" .

core:description a owl:DatatypeProperty ;
    rdfs:comment """This field is a detailed description of the Element. It may also be extracted from the Element itself.
The intent is to provide recipients of the SPDX file with a detailed technical explanation
of the functionality, anticipated use, and anticipated implementation of the Element.
This field may also include a description of improvements over prior versions of the Element.""" ;
    rdfs:domain core:Element ;
    rdfs:range xsd:string ;
    ns0:term_status "Stable" .

core:element a owl:ObjectProperty ;
    rdfs:comment "This field refers to one or more Elements that are part of an ElementCollection." ;
    rdfs:domain core:ElementCollection ;
    rdfs:range core:Element ;
    ns0:term_status "Stable" .

core:end a owl:DatatypeProperty ;
    rdfs:comment "end is a positive integer that defines the end of a range." ;
    rdfs:domain core:PositiveIntegerRange ;
    rdfs:range xsd:positiveInteger ;
    ns0:term_status "Stable" .

core:endTime a owl:DatatypeProperty ;
    rdfs:comment "A endTime specifies the time from which element is no applicable / valid." ;
    rdfs:domain core:Relationship ;
    rdfs:range core:DateTime ;
    ns0:term_status "Stable" .

core:extension rdfs:comment "TODO" ;
    rdfs:domain core:Element ;
    ns0:term_status "Stable" .

core:externalIdentifier a owl:ObjectProperty ;
    rdfs:comment """ExternalIdentifier points to a resource outside the scope of SPDX-3.0 content
that uniquely identifies an Element.""" ;
    rdfs:domain core:Element ;
    rdfs:range core:ExternalIdentifier ;
    ns0:term_status "Stable" .

core:externalIdentifierType a owl:ObjectProperty ;
    rdfs:comment "An externalIdentifierType specifies the type of the external identifier." ;
    rdfs:domain core:ExternalIdentifier ;
    rdfs:range core:ExternalIdentifierType ;
    ns0:term_status "Stable" .

core:externalRef a owl:ObjectProperty ;
    rdfs:comment """This field points to a resource outside the scope of the SPDX-3.0 content
that provides additional characteristics of an Element.""" ;
    rdfs:domain core:Element ;
    rdfs:range core:ExternalRef ;
    ns0:term_status "Stable" .

core:externalRefType a owl:ObjectProperty ;
    rdfs:comment "An externalRefType specifies the type of the external reference." ;
    rdfs:domain core:ExternalRef ;
    rdfs:range core:ExternalRefType ;
    ns0:term_status "Stable" .

core:externalSpdxId a owl:DatatypeProperty ;
    rdfs:comment "ExternalSpdxId identifies an external Element used within a Document but defined external to that Document." ;
    rdfs:domain core:ExternalMap ;
    rdfs:range xsd:anyURI ;
    ns0:term_status "Stable" .

core:from a owl:ObjectProperty ;
    rdfs:comment "This field references the Element on the left-hand side of a relationship." ;
    rdfs:domain core:Relationship ;
    rdfs:range core:Element ;
    ns0:term_status "Stable" .

core:hashValue a owl:DatatypeProperty ;
    rdfs:comment "HashValue is the result of applying a hash algorithm to an Element." ;
    rdfs:domain core:Hash ;
    rdfs:range xsd:string ;
    ns0:term_status "Stable" .

core:identifier a owl:DatatypeProperty ;
    rdfs:comment "An identifier uniquely identifies an external element." ;
    rdfs:domain core:ExternalIdentifier ;
    rdfs:range xsd:string ;
    ns0:term_status "Stable" .

core:identifierLocator a owl:DatatypeProperty ;
    rdfs:comment "A identifierLocator is TODO" ;
    rdfs:domain core:ExternalIdentifier ;
    rdfs:range xsd:anyURI ;
    ns0:term_status "Stable" .

core:imports a owl:ObjectProperty ;
    rdfs:comment """Imports provides an ExternalMap of Element identifiers that are used within a document
but defined external to that document.""" ;
    rdfs:domain core:ElementCollection ;
    rdfs:range core:ExternalMap ;
    ns0:term_status "Stable" .

core:issuingAuthority a owl:DatatypeProperty ;
    rdfs:comment "A issuingAuthority is TODO" ;
    rdfs:domain core:ExternalIdentifier ;
    rdfs:range xsd:anyURI ;
    ns0:term_status "Stable" .

core:key a owl:DatatypeProperty ;
    rdfs:comment """A key used in generic a key-value pair.
A key-value pair can be used to implement a dictionary which associates a key with a value.""" ;
    rdfs:domain core:DictionaryEntry ;
    rdfs:range xsd:string ;
    ns0:term_status "Stable" .

core:locationHint a owl:DatatypeProperty ;
    rdfs:comment "A locationHint provides an indication of where to retrieve an external Element." ;
    rdfs:domain core:ExternalMap ;
    rdfs:range xsd:anyURI ;
    ns0:term_status "Stable" .

core:locator a owl:DatatypeProperty ;
    rdfs:comment "A locator provides the location of an external reference." ;
    rdfs:domain core:ExternalRef ;
    rdfs:range xsd:string ;
    ns0:term_status "Stable" .

core:name a owl:DatatypeProperty ;
    rdfs:comment """This field identifies the name of an Element as designated by the creator. 
The name of an Element is an important convention and easier to refer to than the URI.""" ;
    rdfs:domain core:Element ;
    rdfs:range xsd:string ;
    ns0:term_status "Stable" .

core:originatedBy a owl:ObjectProperty ;
    rdfs:comment "OriginatedBy identifies from where or whom the Element originally came." ;
    rdfs:domain core:Artifact ;
    rdfs:range core:Agent ;
    ns0:term_status "Stable" .

core:profileConformance a owl:ObjectProperty ;
    rdfs:comment """Describes a profile to which the creator of this ElementCollection intends to conform.
The profileConformance will apply to all Elements contained within the collection as well as the collection itself.
Conformance to a profile is defined by the additional restrictions documented in the profile specific documentation and schema files.
Use of this property allows the creator of an ElementCollection to communicate to consumers their intent to adhere to the profile additional restrictions.
The profileConformance has a default value of core if no other profileConformance is specified since all ElementCollections and Element must adhere to the core profile.""" ;
    rdfs:domain core:ElementCollection ;
    rdfs:range core:ProfileIdentifierType ;
    ns0:term_status "Stable" .

core:relationshipType a owl:ObjectProperty ;
    rdfs:comment """This field provides information about the relationship between two Elements.
For example, you can represent a relationship between two different Files,
between a Package and a File, between two Packages, or between one SPDXDocument and another SPDXDocument.""" ;
    rdfs:domain core:Relationship ;
    rdfs:range core:RelationshipType ;
    ns0:term_status "Stable" .

core:releaseTime a owl:DatatypeProperty ;
    rdfs:comment "A releaseTime specifies the time an artifact was released." ;
    rdfs:domain core:Artifact ;
    rdfs:range core:DateTime ;
    ns0:term_status "Stable" .

core:rootElement a owl:ObjectProperty ;
    rdfs:comment """This property is used to denote the root Element(s) of a tree of elements contained in an SBOM.
The tree consists of other elements directly and indirectly related through properties or Relationships from the root.""" ;
    rdfs:domain core:ElementCollection ;
    rdfs:range core:Element ;
    ns0:term_status "Stable" .

core:scope a owl:ObjectProperty ;
    rdfs:comment "A scope is TODO" ;
    rdfs:domain core:LifecycleScopedRelationship ;
    rdfs:range core:LifecycleScopeType ;
    ns0:term_status "Stable" .

core:specVersion a owl:DatatypeProperty ;
    rdfs:comment """The specVersion provides a reference number that can be used to understand how to parse and interpret an Element.
It will enable both future changes to the specification and to support backward compatibility.
The major version number shall be incremented when incompatible changes between versions are made
(one or more sections are created, modified or deleted).
The minor version number shall be incremented when backwards compatible changes are made.

Here, parties exchanging information in accordance with the SPDX specification need to provide 
100% transparency as to which SPDX specification version such information is conforming to.""" ;
    rdfs:domain core:CreationInfo ;
    rdfs:range core:SemVer ;
    ns0:term_status "Stable" .

core:standard a owl:DatatypeProperty ;
    rdfs:comment "Various standards may be relevant to useful to capture for specific artifacts." ;
    rdfs:domain core:Artifact ;
    rdfs:range xsd:string ;
    ns0:term_status "Stable" .

core:startTime a owl:DatatypeProperty ;
    rdfs:comment "A startTime specifies the time from which element is applicable / valid." ;
    rdfs:domain core:Relationship ;
    rdfs:range core:DateTime ;
    ns0:term_status "Stable" .

core:statement a owl:DatatypeProperty ;
    rdfs:comment "A statement is a commentary on an assertion that an annotator has made." ;
    rdfs:domain core:Annotation ;
    rdfs:range xsd:string ;
    ns0:term_status "Stable" .

core:subject a owl:ObjectProperty ;
    rdfs:comment "A subject is an Element an annotator has made an assertion about." ;
    rdfs:domain core:Annotation ;
    rdfs:range core:Element ;
    ns0:term_status "Stable" .

core:summary a owl:DatatypeProperty ;
    rdfs:comment """A summary is a short description of an Element. Here, the intent is to allow the Element creator to 
provide concise information about the function or use of the Element.""" ;
    rdfs:domain core:Element ;
    rdfs:range xsd:string ;
    ns0:term_status "Stable" .

core:suppliedBy a owl:ObjectProperty ;
    rdfs:comment """Identify the actual distribution source for the artifact (e.g., snippet, file, package, vulnerability) or VulnAssessmentRelationship being referenced.
This might or might not be different from the originating distribution source for the artifact (e.g., snippet, file, package, vulnerability) or VulnAssessmentRelationship..""" ;
    rdfs:domain core:Artifact ;
    rdfs:range core:Agent ;
    ns0:term_status "Stable" .

core:to a owl:ObjectProperty ;
    rdfs:comment "This field references an Element on the right-hand side of a relationship." ;
    rdfs:domain core:Relationship ;
    rdfs:range core:Element ;
    ns0:term_status "Stable" .

core:validUntilTime a owl:DatatypeProperty ;
    rdfs:comment "A validUntilTime specifies until when the artifact can be used before its usage needs to be reassessed." ;
    rdfs:domain core:Artifact ;
    rdfs:range core:DateTime ;
    ns0:term_status "Stable" .

core:value a owl:DatatypeProperty ;
    rdfs:comment """A value used in a generic key-value pair.
A key-value pair can be used to implement a dictionary which associates a key with a value.""" ;
    rdfs:domain core:DictionaryEntry ;
    rdfs:range xsd:string ;
    ns0:term_status "Stable" .

<https://spdx.org/rdf/v3/Dataset/ConfidentialityLevelType/amber> a owl:NamedIndividual,
        dataset:ConfidentialityLevelType .

<https://spdx.org/rdf/v3/Dataset/ConfidentialityLevelType/clear> a owl:NamedIndividual,
        dataset:ConfidentialityLevelType .

<https://spdx.org/rdf/v3/Dataset/ConfidentialityLevelType/green> a owl:NamedIndividual,
        dataset:ConfidentialityLevelType .

<https://spdx.org/rdf/v3/Dataset/ConfidentialityLevelType/red> a owl:NamedIndividual,
        dataset:ConfidentialityLevelType .

<https://spdx.org/rdf/v3/Dataset/DatasetAvailabilityType/clickthrough> a owl:NamedIndividual,
        dataset:DatasetAvailabilityType .

<https://spdx.org/rdf/v3/Dataset/DatasetAvailabilityType/directDownload> a owl:NamedIndividual,
        dataset:DatasetAvailabilityType .

<https://spdx.org/rdf/v3/Dataset/DatasetAvailabilityType/query> a owl:NamedIndividual,
        dataset:DatasetAvailabilityType .

<https://spdx.org/rdf/v3/Dataset/DatasetAvailabilityType/registration> a owl:NamedIndividual,
        dataset:DatasetAvailabilityType .

<https://spdx.org/rdf/v3/Dataset/DatasetAvailabilityType/scrapingScript> a owl:NamedIndividual,
        dataset:DatasetAvailabilityType .

<https://spdx.org/rdf/v3/Dataset/DatasetType/audio> a owl:NamedIndividual,
        dataset:DatasetType .

<https://spdx.org/rdf/v3/Dataset/DatasetType/categorical> a owl:NamedIndividual,
        dataset:DatasetType .

<https://spdx.org/rdf/v3/Dataset/DatasetType/graph> a owl:NamedIndividual,
        dataset:DatasetType .

<https://spdx.org/rdf/v3/Dataset/DatasetType/image> a owl:NamedIndividual,
        dataset:DatasetType .

<https://spdx.org/rdf/v3/Dataset/DatasetType/noAssertion> a owl:NamedIndividual,
        dataset:DatasetType .

<https://spdx.org/rdf/v3/Dataset/DatasetType/numeric> a owl:NamedIndividual,
        dataset:DatasetType .

<https://spdx.org/rdf/v3/Dataset/DatasetType/other> a owl:NamedIndividual,
        dataset:DatasetType .

<https://spdx.org/rdf/v3/Dataset/DatasetType/sensor> a owl:NamedIndividual,
        dataset:DatasetType .

<https://spdx.org/rdf/v3/Dataset/DatasetType/structured> a owl:NamedIndividual,
        dataset:DatasetType .

<https://spdx.org/rdf/v3/Dataset/DatasetType/syntactic> a owl:NamedIndividual,
        dataset:DatasetType .

<https://spdx.org/rdf/v3/Dataset/DatasetType/text> a owl:NamedIndividual,
        dataset:DatasetType .

<https://spdx.org/rdf/v3/Dataset/DatasetType/timeseries> a owl:NamedIndividual,
        dataset:DatasetType .

<https://spdx.org/rdf/v3/Dataset/DatasetType/timestamp> a owl:NamedIndividual,
        dataset:DatasetType .

<https://spdx.org/rdf/v3/Dataset/DatasetType/video> a owl:NamedIndividual,
        dataset:DatasetType .

dataset:anonymizationMethodUsed a owl:DatatypeProperty ;
    rdfs:comment "AnonymizationMethodUsed describes the methods used to anonymize the dataset (of fields in the dataset)." ;
    rdfs:domain dataset:Dataset ;
    rdfs:range xsd:string ;
    ns0:term_status "Stable" .

dataset:confidentialityLevel a owl:ObjectProperty ;
    rdfs:comment "ConfidentialityLevel describes the levels of confidentiality of the data points contained in the dataset." ;
    rdfs:domain dataset:Dataset ;
    rdfs:range dataset:ConfidentialityLevelType ;
    ns0:term_status "Stable" .

dataset:dataCollectionProcess a owl:DatatypeProperty ;
    rdfs:comment """DataCollectionProcess describes how a dataset was collected.
Examples include the sources from which a dataset was scrapped or
the interview protocol that was used for data collection.""" ;
    rdfs:domain dataset:Dataset ;
    rdfs:range xsd:string ;
    ns0:term_status "Stable" .

dataset:dataPreprocessing a owl:DatatypeProperty ;
    rdfs:comment """DataPreprocessing describes the various preprocessing steps
that were applied to the raw data to create the dataset.""" ;
    rdfs:domain dataset:Dataset ;
    rdfs:range xsd:string ;
    ns0:term_status "Stable" .

dataset:datasetAvailability a owl:DatatypeProperty ;
    rdfs:comment "Some datasets are publicly available and can be downloaded directly. Others are only accessible behind a clickthrough, or after filling a registration form. This field will describe the dataset availability from that perspective." ;
    rdfs:domain dataset:Dataset ;
    rdfs:range dataset:DatasetAvailabilityType ;
    ns0:term_status "Stable" .

dataset:datasetNoise a owl:DatatypeProperty ;
    rdfs:comment """DatasetNoise describes what kinds of noises a dataset might encompass.
The field uses free form text to specify the fields or the samples that might be noisy.
Alternatively, it can also be used to describe various noises that could impact the whole dataset.""" ;
    rdfs:domain dataset:Dataset ;
    rdfs:range xsd:string ;
    ns0:term_status "Stable" .

dataset:datasetSize a owl:DatatypeProperty ;
    rdfs:comment """DatasetSize Captures how large a dataset is.
The size is to be measured in bytes.""" ;
    rdfs:domain dataset:Dataset ;
    rdfs:range xsd:nonNegativeInteger ;
    ns0:term_status "Stable" .

dataset:datasetType a owl:DatatypeProperty ;
    rdfs:comment "Type describes the datatype contained in the dataset. For example a dataset can be an image dataset for computer vision applications, a text dataset such as the contents of a book or Wikipedia article, or sometimes a multimodal dataset that contains multiple types of data." ;
    rdfs:domain dataset:Dataset ;
    rdfs:range dataset:DatasetType ;
    ns0:term_status "Stable" .

dataset:datasetUpdateMechanism a owl:DatatypeProperty ;
    rdfs:comment "DatasetUpdateMechanism describes a mechanism to update the dataset." ;
    rdfs:domain dataset:Dataset ;
    rdfs:range xsd:string ;
    ns0:term_status "Stable" .

dataset:intendedUse a owl:DatatypeProperty ;
    rdfs:comment """IntendedUse describes what the given dataset should be used for.
Some datasets are collected to be used only for particular purposes. 
For example, medical data collected from a specific demography might only be applicable
for training machine learning models to make predictions for that demography.
In such a case, the intendedUse field would capture this information.
Similarly, if a dataset is collected for building a facial recognition model,
the intendedUse field would specify that.""" ;
    rdfs:domain dataset:Dataset ;
    rdfs:range xsd:string ;
    ns0:term_status "Stable" .

dataset:knownBias a owl:DatatypeProperty ;
    rdfs:comment "KnownBias is a free form text field that describes the different biases that the dataset encompasses." ;
    rdfs:domain dataset:Dataset ;
    rdfs:range xsd:string ;
    ns0:term_status "Stable" .

dataset:sensitivePersonalInformation a owl:ObjectProperty ;
    rdfs:comment """SensitivePersonalInformation indicates the presence of sensitive personal data
or information that allows drawing conclusions about a person's identity.""" ;
    rdfs:domain dataset:Dataset ;
    rdfs:range core:PresenceType ;
    ns0:term_status "Stable" .

dataset:sensor a owl:ObjectProperty ;
    rdfs:comment """Sensor describes a sensor that was used for collecting the data
and its calibration value as a key-value pair.""" ;
    rdfs:domain dataset:Dataset ;
    rdfs:range core:DictionaryEntry ;
    ns0:term_status "Stable" .

expandedlicensing:ConjunctiveLicenseSet a owl:Class,
        sh:NodeShape ;
    rdfs:comment """A ConjunctiveLicenseSet indicates that _each_ of its subsidiary
AnyLicenseInfos apply. In other words, a ConjunctiveLicenseSet of two or
more licenses represents a licensing situation where _all_ of the specified
licenses are to be complied with. It is represented in the SPDX License
Expression Syntax by the `AND` operator.

It is syntactically correct to specify a ConjunctiveLicenseSet where the
subsidiary AnyLicenseInfos may be "incompatible" according to a particular
interpretation of the corresponding Licenses. The SPDX License Expression
Syntax does not take into account interpretation of license texts, which is
left to the consumer of SPDX data to determine for themselves.""" ;
    rdfs:subClassOf simplelicensing:AnyLicenseInfo ;
    ns0:term_status "Stable" ;
    sh:property [ sh:class simplelicensing:AnyLicenseInfo ;
            sh:minCount 2 ;
            sh:name "member" ;
            sh:path expandedlicensing:member ] .

expandedlicensing:DisjunctiveLicenseSet a owl:Class,
        sh:NodeShape ;
    rdfs:comment """A DisjunctiveLicenseSet indicates that _only one_ of its subsidiary
AnyLicenseInfos is required to apply. In other words, a
DisjunctiveLicenseSet of two or more licenses represents a licensing
situation where _only one_ of the specified licenses are to be complied with.
A consumer of SPDX data would typically understand this to permit the recipient
of the licensed content to choose which of the corresponding license they
would prefer to use. It is represented in the SPDX License Expression Syntax
by the `OR` operator.""" ;
    rdfs:subClassOf simplelicensing:AnyLicenseInfo ;
    ns0:term_status "Stable" ;
    sh:property [ sh:class simplelicensing:AnyLicenseInfo ;
            sh:minCount 2 ;
            sh:name "member" ;
            sh:path expandedlicensing:member ] .

expandedlicensing:OrLaterOperator a owl:Class,
        sh:NodeShape ;
    rdfs:comment """An OrLaterOperator indicates that this portion of the AnyLicenseInfo
represents either (1) the specified version of the corresponding License, or
(2) any later version of that License. It is represented in the SPDX License
Expression Syntax by the `+` operator.

It is context-dependent, and unspecified by SPDX, as to what constitutes a
"later version" of any particular License. Some Licenses may not be versioned,
or may not have clearly-defined ordering for versions. The consumer of SPDX
data will need to determine for themselves what meaning to attribute to a
"later version" operator for a particular License.""" ;
    rdfs:subClassOf expandedlicensing:ExtendableLicense ;
    ns0:term_status "Stable" ;
    sh:property [ sh:class expandedlicensing:License ;
            sh:maxCount 1 ;
            sh:minCount 1 ;
            sh:name "subjectLicense" ;
            sh:path expandedlicensing:subjectLicense ] .

expandedlicensing:additionText a owl:DatatypeProperty ;
    rdfs:comment """An additionText contains the plain text of the LicenseAddition, without
templating or other similar markup.

Users of the additionText for a License can apply the SPDX Matching Guidelines
when comparing it to another text for matching purposes.""" ;
    rdfs:domain expandedlicensing:LicenseAddition ;
    rdfs:range xsd:string ;
    ns0:term_status "Stable" .

expandedlicensing:isDeprecatedAdditionId a owl:DatatypeProperty ;
    rdfs:comment """The isDeprecatedAdditionId property specifies whether an identifier for a
LicenseAddition has been marked as deprecated. If the property is not defined,
then it is presumed to be false (i.e., not deprecated).

If the LicenseAddition is included on the SPDX Exceptions List, then
the `deprecatedVersion` property indicates on which version release of the
Exceptions List it was first marked as deprecated.

"Deprecated" in this context refers to deprecating the use of the
_identifier_, not the underlying license addition. In other words, even if a
LicenseAddition's author or steward has stated that a particular
LicenseAddition generally should not be used, that would _not_ mean that the
LicenseAddition's identifier is "deprecated." Rather, a LicenseAddition
operator is typically marked as "deprecated" when it is determined that use of
another identifier is preferable.""" ;
    rdfs:domain expandedlicensing:LicenseAddition ;
    rdfs:range xsd:boolean ;
    ns0:term_status "Stable" .

expandedlicensing:isDeprecatedLicenseId a owl:DatatypeProperty ;
    rdfs:comment """The isDeprecatedLicenseId property specifies whether an identifier for a
License or LicenseAddition has been marked as deprecated. If the property
is not defined, then it is presumed to be false (i.e., not deprecated).

If the License or LicenseAddition is included on the SPDX License List, then
the `deprecatedVersion` property indicates on which version release of the
License List it was first marked as deprecated.

"Deprecated" in this context refers to deprecating the use of the
_identifier_, not the underlying license. In other words, even if a License's
author or steward has stated that a particular License generally should not be
used, that would _not_ mean that the License's identifier is "deprecated."
Rather, a License or LicenseAddition operator is typically marked as
"deprecated" when it is determined that use of another identifier is
preferable.""" ;
    rdfs:domain expandedlicensing:License ;
    rdfs:range xsd:boolean ;
    ns0:term_status "Stable" .

expandedlicensing:isFsfLibre a owl:DatatypeProperty ;
    rdfs:comment """isFsfLibre specifies whether the [Free Software Foundation FSF](https://fsf.org)
has listed this License as "free" in their commentary on licenses, located at
the time of this writing at https://www.gnu.org/licenses/license-list.en.html.

A value of "true" indicates that the license is in the list of licenses that FSF publishes as libre.

A value of "false" indicates that the license is explicitly not in the corresponding list of FSF libre licenses (e.g., FSF has the license on a non-free list).

If the isFsfLibre field is not specified, the SPDX data creator makes no
assertions about whether the License is listed in the FSF's commentary.""" ;
    rdfs:domain expandedlicensing:License ;
    rdfs:range xsd:boolean ;
    ns0:term_status "Stable" .

expandedlicensing:isOsiApproved a owl:DatatypeProperty ;
    rdfs:comment """isOsiApproved specifies whether the [Open Source Initiative (OSI)](https://opensource.org)
has listed this License as "approved" in their list of OSI Approved Licenses,
located at the time of this writing at https://opensource.org/licenses/.

A value of "true" indicates that the license is in the list of licenses that OSI publishes as approved.

A value of "false" indicates that the license is explicitly not in the corresponding list of OSI licenses (e.g., OSI has stated publicly that a license is not approved).

If the isOsiApproved field is not specified, the SPDX data creator makes no
assertions about whether the License is approved by the OSI.""" ;
    rdfs:domain expandedlicensing:License ;
    rdfs:range xsd:boolean ;
    ns0:term_status "Stable" .

expandedlicensing:standardAdditionTemplate a owl:DatatypeProperty ;
    rdfs:comment """A standardAdditionTemplate contains a license addition template which describes
sections of the LicenseAddition text which can be varied. See the Legacy Text
Template format section of the SPDX specification for format information.""" ;
    rdfs:domain expandedlicensing:LicenseAddition ;
    rdfs:range xsd:string ;
    ns0:term_status "Stable" .

expandedlicensing:standardLicenseHeader a owl:DatatypeProperty ;
    rdfs:comment """A standardLicenseHeader contains the plain text of the License author's
preferred wording to be used, typically in a source code file's header
comments or similar location, to indicate that the file is subject to
the specified License.""" ;
    rdfs:domain expandedlicensing:License ;
    rdfs:range xsd:string ;
    ns0:term_status "Stable" .

expandedlicensing:standardLicenseTemplate a owl:DatatypeProperty ;
    rdfs:comment """A standardLicenseTemplate contains a license template which describes
sections of the License text which can be varied. See the Legacy Text Template
format section of the SPDX specification for format information.""" ;
    rdfs:domain expandedlicensing:License ;
    rdfs:range xsd:string ;
    ns0:term_status "Stable" .

expandedlicensing:subjectAddition a owl:ObjectProperty ;
    rdfs:comment """A subjectAddition is a LicenseAddition which is subject to a 'with additional
text' effect (WithAdditionOperator).""" ;
    rdfs:domain expandedlicensing:WithAdditionOperator ;
    rdfs:range expandedlicensing:LicenseAddition ;
    ns0:term_status "Stable" .

<https://spdx.org/rdf/v3/Security/CvssSeverityType/critical> a owl:NamedIndividual,
        security:CvssSeverityType .

<https://spdx.org/rdf/v3/Security/CvssSeverityType/high> a owl:NamedIndividual,
        security:CvssSeverityType .

<https://spdx.org/rdf/v3/Security/CvssSeverityType/low> a owl:NamedIndividual,
        security:CvssSeverityType .

<https://spdx.org/rdf/v3/Security/CvssSeverityType/medium> a owl:NamedIndividual,
        security:CvssSeverityType .

<https://spdx.org/rdf/v3/Security/CvssSeverityType/none> a owl:NamedIndividual,
        security:CvssSeverityType .

<https://spdx.org/rdf/v3/Security/ExploitCatalogType/kev> a owl:NamedIndividual,
        security:ExploitCatalogType .

<https://spdx.org/rdf/v3/Security/ExploitCatalogType/other> a owl:NamedIndividual,
        security:ExploitCatalogType .

<https://spdx.org/rdf/v3/Security/SsvcDecisionType/act> a owl:NamedIndividual,
        security:SsvcDecisionType .

<https://spdx.org/rdf/v3/Security/SsvcDecisionType/attend> a owl:NamedIndividual,
        security:SsvcDecisionType .

<https://spdx.org/rdf/v3/Security/SsvcDecisionType/track> a owl:NamedIndividual,
        security:SsvcDecisionType .

<https://spdx.org/rdf/v3/Security/SsvcDecisionType/trackStar> a owl:NamedIndividual,
        security:SsvcDecisionType .

security:SsvcVulnAssessmentRelationship a owl:Class,
        sh:NodeShape ;
    rdfs:comment """An SsvcVulnAssessmentRelationship describes the decision made using the
Stakeholder-Specific Vulnerability Categorization (SSVC) decision tree as
defined on [https://www.cisa.gov/stakeholder-specific-vulnerability-categorization-ssvc](https://www.cisa.gov/stakeholder-specific-vulnerability-categorization-ssvc).
It is intended to communicate the results of using the CISA SSVC Calculator.

**Constraints**

- The relationship type must be set to hasAssessmentFor.

**Syntax**

```json
{
  "@type": "SsvcVulnAssessmentRelationship",
  "@id": "urn:spdx.dev:ssvc-1",
  "relationshipType": "hasAssessmentFor",
  "decisionType": "act",
  "from": "urn:spdx.dev:vuln-cve-2020-28498",
  "to": ["urn:product-acme-application-1.3"],
  "assessedElement": "urn:npm-elliptic-6.5.2",
  "suppliedBy": ["urn:spdx.dev:agent-jane-doe"],
  "publishedTime": "2021-03-09T11:04:53Z"
}
```""" ;
    rdfs:subClassOf security:VulnAssessmentRelationship ;
    ns0:term_status "Stable" ;
    sh:property [ sh:class security:SsvcDecisionType ;
            sh:maxCount 1 ;
            sh:minCount 1 ;
            sh:name "decisionType" ;
            sh:path security:decisionType ] .

<https://spdx.org/rdf/v3/Security/VexJustificationType/componentNotPresent> a owl:NamedIndividual,
        security:VexJustificationType .

<https://spdx.org/rdf/v3/Security/VexJustificationType/inlineMitigationsAlreadyExist> a owl:NamedIndividual,
        security:VexJustificationType .

<https://spdx.org/rdf/v3/Security/VexJustificationType/vulnerableCodeCannotBeControlledByAdversary> a owl:NamedIndividual,
        security:VexJustificationType .

<https://spdx.org/rdf/v3/Security/VexJustificationType/vulnerableCodeNotInExecutePath> a owl:NamedIndividual,
        security:VexJustificationType .

<https://spdx.org/rdf/v3/Security/VexJustificationType/vulnerableCodeNotPresent> a owl:NamedIndividual,
        security:VexJustificationType .

security:actionStatement a owl:DatatypeProperty ;
    rdfs:comment """When an element is referenced with a VexAffectedVulnAssessmentRelationship,
the relationship MUST include one actionStatement that SHOULD describe actions
to remediate or mitigate the vulnerability.""" ;
    rdfs:domain security:VexAffectedVulnAssessmentRelationship ;
    rdfs:range xsd:string ;
    ns0:term_status "Stable" .

security:actionStatementTime a owl:DatatypeProperty ;
    rdfs:comment """When a VEX statement communicates an affected status, the author MUST
include an action statement with a recommended action to help mitigate the
vulnerability's impact. The actionStatementTime property records the time
when the action statement was first communicated.""" ;
    rdfs:domain security:VexAffectedVulnAssessmentRelationship ;
    rdfs:range core:DateTime ;
    ns0:term_status "Stable" .

security:assessedElement a owl:ObjectProperty ;
    rdfs:comment """Specifies subpackages, files or snippets referenced by a security assessment
to specify the precise location where a vulnerability was found.""" ;
    rdfs:domain security:VulnAssessmentRelationship ;
    rdfs:range core:Element ;
    ns0:term_status "Stable" .

security:catalogType a owl:ObjectProperty ;
    rdfs:comment "A catalogType is a mandatory value and must select one of the two entries in the `ExploitCatalogType.md` vocabulary." ;
    rdfs:domain security:ExploitCatalogVulnAssessmentRelationship ;
    rdfs:range security:ExploitCatalogType ;
    ns0:term_status "Stable" .

security:decisionType a owl:ObjectProperty ;
    rdfs:comment "A decisionType is a mandatory value and must select one of the four entries in the `SsvcDecisionType.md` vocabulary." ;
    rdfs:domain security:SsvcVulnAssessmentRelationship ;
    rdfs:range security:SsvcDecisionType ;
    ns0:term_status "Stable" .

security:exploited a owl:DatatypeProperty ;
    rdfs:comment "This field is set when a CVE is listed in an exploit catalog." ;
    rdfs:domain security:ExploitCatalogVulnAssessmentRelationship ;
    rdfs:range xsd:boolean ;
    ns0:term_status "Stable" .

security:impactStatement a owl:DatatypeProperty ;
    rdfs:comment """When a VEX product element is related with a VexNotAffectedVulnAssessmentRelationship
and a machine readable justification label is not provided, then an impactStatement
that further explains how or why the prouct(s) are not affected by the vulnerability
must be provided.""" ;
    rdfs:domain security:VexNotAffectedVulnAssessmentRelationship ;
    rdfs:range xsd:string ;
    ns0:term_status "Stable" .

security:impactStatementTime a owl:DatatypeProperty ;
    rdfs:comment "TODO" ;
    rdfs:domain security:VexNotAffectedVulnAssessmentRelationship ;
    rdfs:range core:DateTime ;
    ns0:term_status "Stable" .

security:justificationType a owl:ObjectProperty ;
    rdfs:comment """When stating that an element is not affected by a vulnerability, the
VexNotAffectedVulnAssessmentRelationship must include a justification from the
machine-readable labels catalog informing the reason the element is not impacted.

impactStatement which is a string with English prose can be used instead or as
complementary to the justification label, but one of both MUST be defined.""" ;
    rdfs:domain security:VexNotAffectedVulnAssessmentRelationship ;
    rdfs:range security:VexJustificationType ;
    ns0:term_status "Stable" .

security:locator a owl:DatatypeProperty ;
    rdfs:comment "A locator provides the location of an exploit catalog." ;
    rdfs:domain security:ExploitCatalogVulnAssessmentRelationship ;
    rdfs:range xsd:anyURI ;
    ns0:term_status "Stable" .

security:percentile a owl:DatatypeProperty ;
    rdfs:comment "The percentile between 0 and 1 (0 and 100%) of the current probability score, the proportion of all scored vulnerabilities with the same or a lower EPSS score. [https://www.first.org/epss/data_stats](https://www.first.org/epss/data_stats)" ;
    rdfs:domain security:EpssVulnAssessmentRelationship ;
    rdfs:range xsd:decimal ;
    ns0:term_status "Stable" .

security:probability a owl:DatatypeProperty ;
    rdfs:comment "The probability score between 0 and 1 (0 and 100%) estimating the likelihood of exploitation in the wild in the next 30 days (following score publication). [https://www.first.org/epss/data_stats](https://www.first.org/epss/data_stats)" ;
    rdfs:domain security:EpssVulnAssessmentRelationship ;
    rdfs:range xsd:decimal ;
    ns0:term_status "Stable" .

security:statusNotes a owl:DatatypeProperty ;
    rdfs:comment "TODO" ;
    rdfs:domain security:VexVulnAssessmentRelationship ;
    rdfs:range xsd:string ;
    ns0:term_status "Stable" .

security:suppliedBy a owl:ObjectProperty ;
    rdfs:comment "Identify the actual distribution source for the vulnerability assessment relationship being referenced." ;
    rdfs:domain security:VulnAssessmentRelationship ;
    rdfs:range core:Agent ;
    ns0:term_status "Stable" .

security:vexVersion a owl:DatatypeProperty ;
    rdfs:comment "TODO" ;
    rdfs:domain security:VexVulnAssessmentRelationship ;
    rdfs:range xsd:string ;
    ns0:term_status "Stable" .

simplelicensing:SimpleLicensingText a owl:Class,
        sh:NodeShape ;
    rdfs:comment """A SimpleLicensingText represents a License or Addition that is not listed on the SPDX License
List at https://spdx.org/licenses, and is therefore defined by an SPDX data
creator.""" ;
    rdfs:subClassOf core:Element ;
    ns0:term_status "Stable" ;
    sh:property [ sh:datatype xsd:string ;
            sh:maxCount 1 ;
            sh:minCount 1 ;
            sh:name "licenseText" ;
            sh:path simplelicensing:licenseText ] .

simplelicensing:customIdToUri a owl:ObjectProperty ;
    rdfs:comment """Within a License Expression, references can be made to a Custom License or a Custom License Addition.
The License Expression syntax dictates any refence starting with a "LicenseRef-" or "AdditionRef-" refers to license or addition text not found in the SPDX list of licenses.
These custom licenses must be a CustomLicense, a CustomLicenseAddtion, or a SimpleLicensingText which are identified with a unique URI identifier.
The key for the DictionaryEntry is the string used in the license expression and the value is the URI for the corrosponding CustomLicense, CustomLicenseAddition, or SimpleLicensingText.""" ;
    rdfs:domain simplelicensing:LicenseExpression ;
    rdfs:range core:DictionaryEntry ;
    ns0:term_status "Stable" .

simplelicensing:licenseExpression a owl:DatatypeProperty ;
    rdfs:comment """Often a single license can be used to represent the licensing terms of a source code or binary file, but there are situations where a single license identifier is not sufficient. A common example is when software is offered under a choice of one or more licenses (e.g., GPL-2.0-only OR BSD-3-Clause). Another example is when a set of licenses is needed to represent a binary program constructed by compiling and linking two (or more) different source files each governed by different licenses (e.g., LGPL-2.1-only AND BSD-3-Clause).

SPDX License Expressions provide a way for one to construct expressions that more accurately represent the licensing terms typically found in open source software source code. A license expression could be a single license identifier found on the SPDX License List; a user defined license reference denoted by the LicenseRef-idString; a license identifier combined with an SPDX exception; or some combination of license identifiers, license references and exceptions constructed using a small set of defined operators (e.g., AND, OR, WITH and +). We provide the definition of what constitutes a valid an SPDX License Expression in this section.""" ;
    rdfs:domain simplelicensing:LicenseExpression ;
    rdfs:range xsd:string ;
    ns0:term_status "Stable" .

simplelicensing:licenseListVersion a owl:DatatypeProperty ;
    rdfs:comment """Recognizing that licenses are added to the SPDX License List with each subsequent version, the intent is to provide consumers with the version of the SPDX License List used. 
This anticipates that in the future, license expression might have used a version of the SPDX License List that is older than the then current one.
The specified version of the SPDX License List must include all listed licenses and exceptions referenced in the expression.""" ;
    rdfs:domain simplelicensing:LicenseExpression ;
    rdfs:range core:SemVer ;
    ns0:term_status "Stable" .

<https://spdx.org/rdf/v3/Software/DependencyConditionalityType/optional> a owl:NamedIndividual,
        software:DependencyConditionalityType .

<https://spdx.org/rdf/v3/Software/DependencyConditionalityType/other> a owl:NamedIndividual,
        software:DependencyConditionalityType .

<https://spdx.org/rdf/v3/Software/DependencyConditionalityType/prerequisite> a owl:NamedIndividual,
        software:DependencyConditionalityType .

<https://spdx.org/rdf/v3/Software/DependencyConditionalityType/provided> a owl:NamedIndividual,
        software:DependencyConditionalityType .

<https://spdx.org/rdf/v3/Software/DependencyConditionalityType/required> a owl:NamedIndividual,
        software:DependencyConditionalityType .

software:Sbom a owl:Class,
        sh:NodeShape ;
    rdfs:comment """A Software Bill of Materials (SBOM) is a collection of SPDX Elements describing a single package.
This could include details of the content and composition of the product,
provenance details of the product and/or
its composition, licensing information, known quality or security issues, etc.""" ;
    rdfs:subClassOf core:Bom ;
    ns0:term_status "Stable" ;
    sh:property [ sh:class software:SbomType ;
            sh:name "sbomType" ;
            sh:path software:sbomType ] .

<https://spdx.org/rdf/v3/Software/SbomType/analyzed> a owl:NamedIndividual,
        software:SbomType .

<https://spdx.org/rdf/v3/Software/SbomType/build> a owl:NamedIndividual,
        software:SbomType .

<https://spdx.org/rdf/v3/Software/SbomType/deployed> a owl:NamedIndividual,
        software:SbomType .

<https://spdx.org/rdf/v3/Software/SbomType/design> a owl:NamedIndividual,
        software:SbomType .

<https://spdx.org/rdf/v3/Software/SbomType/runtime> a owl:NamedIndividual,
        software:SbomType .

<https://spdx.org/rdf/v3/Software/SbomType/source> a owl:NamedIndividual,
        software:SbomType .

<https://spdx.org/rdf/v3/Software/SoftwareDependencyLinkType/dynamic> a owl:NamedIndividual,
        software:SoftwareDependencyLinkType .

<https://spdx.org/rdf/v3/Software/SoftwareDependencyLinkType/other> a owl:NamedIndividual,
        software:SoftwareDependencyLinkType .

<https://spdx.org/rdf/v3/Software/SoftwareDependencyLinkType/static> a owl:NamedIndividual,
        software:SoftwareDependencyLinkType .

<https://spdx.org/rdf/v3/Software/SoftwareDependencyLinkType/tool> a owl:NamedIndividual,
        software:SoftwareDependencyLinkType .

<https://spdx.org/rdf/v3/Software/SoftwarePurpose/application> a owl:NamedIndividual,
        software:SoftwarePurpose .

<https://spdx.org/rdf/v3/Software/SoftwarePurpose/archive> a owl:NamedIndividual,
        software:SoftwarePurpose .

<https://spdx.org/rdf/v3/Software/SoftwarePurpose/bom> a owl:NamedIndividual,
        software:SoftwarePurpose .

<https://spdx.org/rdf/v3/Software/SoftwarePurpose/configuration> a owl:NamedIndividual,
        software:SoftwarePurpose .

<https://spdx.org/rdf/v3/Software/SoftwarePurpose/container> a owl:NamedIndividual,
        software:SoftwarePurpose .

<https://spdx.org/rdf/v3/Software/SoftwarePurpose/data> a owl:NamedIndividual,
        software:SoftwarePurpose .

<https://spdx.org/rdf/v3/Software/SoftwarePurpose/device> a owl:NamedIndividual,
        software:SoftwarePurpose .

<https://spdx.org/rdf/v3/Software/SoftwarePurpose/deviceDriver> a owl:NamedIndividual,
        software:SoftwarePurpose .

<https://spdx.org/rdf/v3/Software/SoftwarePurpose/diskImage> a owl:NamedIndividual,
        software:SoftwarePurpose .

<https://spdx.org/rdf/v3/Software/SoftwarePurpose/documentation> a owl:NamedIndividual,
        software:SoftwarePurpose .

<https://spdx.org/rdf/v3/Software/SoftwarePurpose/evidence> a owl:NamedIndividual,
        software:SoftwarePurpose .

<https://spdx.org/rdf/v3/Software/SoftwarePurpose/executable> a owl:NamedIndividual,
        software:SoftwarePurpose .

<https://spdx.org/rdf/v3/Software/SoftwarePurpose/file> a owl:NamedIndividual,
        software:SoftwarePurpose .

<https://spdx.org/rdf/v3/Software/SoftwarePurpose/filesystemImage> a owl:NamedIndividual,
        software:SoftwarePurpose .

<https://spdx.org/rdf/v3/Software/SoftwarePurpose/firmware> a owl:NamedIndividual,
        software:SoftwarePurpose .

<https://spdx.org/rdf/v3/Software/SoftwarePurpose/framework> a owl:NamedIndividual,
        software:SoftwarePurpose .

<https://spdx.org/rdf/v3/Software/SoftwarePurpose/install> a owl:NamedIndividual,
        software:SoftwarePurpose .

<https://spdx.org/rdf/v3/Software/SoftwarePurpose/library> a owl:NamedIndividual,
        software:SoftwarePurpose .

<https://spdx.org/rdf/v3/Software/SoftwarePurpose/manifest> a owl:NamedIndividual,
        software:SoftwarePurpose .

<https://spdx.org/rdf/v3/Software/SoftwarePurpose/model> a owl:NamedIndividual,
        software:SoftwarePurpose .

<https://spdx.org/rdf/v3/Software/SoftwarePurpose/module> a owl:NamedIndividual,
        software:SoftwarePurpose .

<https://spdx.org/rdf/v3/Software/SoftwarePurpose/operatingSystem> a owl:NamedIndividual,
        software:SoftwarePurpose .

<https://spdx.org/rdf/v3/Software/SoftwarePurpose/other> a owl:NamedIndividual,
        software:SoftwarePurpose .

<https://spdx.org/rdf/v3/Software/SoftwarePurpose/patch> a owl:NamedIndividual,
        software:SoftwarePurpose .

<https://spdx.org/rdf/v3/Software/SoftwarePurpose/platform> a owl:NamedIndividual,
        software:SoftwarePurpose .

<https://spdx.org/rdf/v3/Software/SoftwarePurpose/requirement> a owl:NamedIndividual,
        software:SoftwarePurpose .

<https://spdx.org/rdf/v3/Software/SoftwarePurpose/source> a owl:NamedIndividual,
        software:SoftwarePurpose .

<https://spdx.org/rdf/v3/Software/SoftwarePurpose/specification> a owl:NamedIndividual,
        software:SoftwarePurpose .

<https://spdx.org/rdf/v3/Software/SoftwarePurpose/test> a owl:NamedIndividual,
        software:SoftwarePurpose .

software:additionalPurpose a owl:ObjectProperty ;
    rdfs:comment "Additional purpose provides information about the additional purposes of the software artifact in addition to the primaryPurpose." ;
    rdfs:domain software:SoftwareArtifact ;
    rdfs:range software:SoftwarePurpose ;
    ns0:term_status "Stable" .

software:attributionText a owl:DatatypeProperty ;
    rdfs:comment """An attributionText for a software Package, File or Snippet provides a consumer
of SPDX data with acknowledgement content, to assist redistributors of the
Package, File or Snippet with reproducing those acknowledgements.

For example, this field may include a statement that is required by a
particular license to be reproduced in end-user documentation, advertising
materials, or another form.

This field may describe where, or in which contexts, the acknowledgements
need to be reproduced, but it is not required to do so. The SPDX data creator
may also explain elsewhere (such as in a licenseComment field) how they intend
for data in this field to be used.

An attributionText is is not meant to include the software Package, File or
Snippet’s actual complete license text (see concludedLicense to identify the
corresponding license).""" ;
    rdfs:domain software:SoftwareArtifact ;
    rdfs:range xsd:string ;
    ns0:term_status "Stable" .

software:byteRange a owl:DatatypeProperty ;
    rdfs:comment """This field defines the byte range in the original host file that the snippet information applies to.
A range of bytes is independent of various formatting concerns, and the most accurate way 
of referring to the differences. The choice was made to start the numbering of 
the byte range at 1 to be consistent with the W3C pointer method vocabulary.""" ;
    rdfs:domain software:Snippet ;
    rdfs:range core:PositiveIntegerRange ;
    ns0:term_status "Stable" .

software:conditionality a owl:ObjectProperty ;
    rdfs:comment "A conditionality is TODO" ;
    rdfs:domain software:SoftwareDependencyRelationship ;
    rdfs:range software:DependencyConditionalityType ;
    ns0:term_status "Stable" .

software:contentIdentifier a owl:DatatypeProperty ;
    rdfs:comment """The contentIdentifier provides a canonical, unique, immutable artifact identifier for each software artifact. SPDX 3.0 describes software artifacts as Snippet, File, or Package Elements. The ContentIdentifier can be calculated for any software artifact and can be recorded for any of these SPDX 3.0 Elements using Omnibor, an attempt to standardize how software artifacts are identified independent of which programming language, version control system, build tool, package manager, or software distribution mechanism is in use.  

The contentIdentifier is defined as the [Git Object Identifier](https://git-scm.com/book/en/v2/Git-Internals-Git-Objects) (gitoid) of type `blob` of the software artifact. The use of a git-based version control system is not necessary to calculate a contentIdentifier for any software artifact.

The gitoid is expressed in the ContentIdentifier property by using the IANA [gitoid URI scheme](https://www.iana.org/assignments/uri-schemes/prov/gitoid).

```
Scheme syntax: gitoid":"<git object type>":"<hash algorithm>":"<hash value>
```

The OmniBOR ID for the OmniBOR Document associated with a software artifact should not be recorded in this field. Rather, OmniBOR IDs should be recorded in the SPDX Element's ExternalIdentifier property. See [https://omnibor.io](https://omnibor.io) for more details.""" ;
    rdfs:domain software:SoftwareArtifact ;
    rdfs:range xsd:anyURI ;
    ns0:term_status "Stable" .

software:contentType a owl:DatatypeProperty ;
    rdfs:comment """This field is a reasonable estimation of the content type of the Element, from a creator perspective.
Content type is intrinsic to the Element, independent of how the Element is being used.""" ;
    rdfs:domain software:File ;
    rdfs:range core:MediaType ;
    ns0:term_status "Stable" .

software:copyrightText a owl:DatatypeProperty ;
    rdfs:comment """A copyrightText consists of the text(s) of the copyright notice(s) found
for a software Package, File or Snippet, if any.

If a copyrightText contains text, then it may contain any text related to
one or more copyright notices (even if not complete) for that software
Package, File or Snippet.

If a copyrightText has a "NONE" value, this indicates that the software
Package, File or Snippet contains no copyright notice whatsoever.

If a copyrightText has a "NOASSERTION" value, this indicates that one of the
following applies:
* the SPDX data creator has attempted to but cannot reach a reasonable
  objective determination;
* the SPDX data creator has made no attempt to determine this field; or
* the SPDX data creator has intentionally provided no information (no
  meaning should be implied by doing so).""" ;
    rdfs:domain software:SoftwareArtifact ;
    rdfs:range xsd:string ;
    ns0:term_status "Stable" .

software:downloadLocation a owl:DatatypeProperty ;
    rdfs:comment """DownloadLocation identifies the download Uniform Resource Identifier 
for the package at the time that the document was created.
Where and how to download the exact package being referenced 
is critical for verification and tracking data.""" ;
    rdfs:domain software:Package ;
    rdfs:range xsd:anyURI ;
    ns0:term_status "Stable" .

software:homePage a owl:DatatypeProperty ;
    rdfs:comment """HomePage is a place for the SPDX document creator to record a website that serves as the package's home page.
This saves the recipient of the SPDX document who is looking for more info from
having to search for and verify a match between the package and the associated project home page.
This link can also be used to reference further information about the package
referenced by the SPDX document creator.""" ;
    rdfs:domain software:Package ;
    rdfs:range xsd:anyURI ;
    ns0:term_status "Stable" .

software:lineRange a owl:DatatypeProperty ;
    rdfs:comment """This field defines the line range in the original host file that the snippet information applies to.
If there is a disagreement between the byte range and line range, the byte range values will take precedence.
A range of lines is a convenient reference for those files where there is a known line delimiter. 
The choice was made to start the numbering of the lines at 1 to be consistent with the W3C pointer method vocabulary.""" ;
    rdfs:domain software:Snippet ;
    rdfs:range core:PositiveIntegerRange ;
    ns0:term_status "Stable" .

software:packageUrl a owl:DatatypeProperty ;
    rdfs:comment """A packageUrl (commonly pronounced and referred to as "purl") is an attempt to standardize package representations in order to reliably identify and locate software packages. A purl is a URL string which represents a package in a mostly universal and uniform way across programming languages, package managers, packaging conventions, tools, APIs and databases.

the purl URL string is defined by seven components:
```
scheme:type/namespace/name@version?qualifiers#subpath
```

The definition for each component can be found in the [purl specification](https://github.com/package-url/purl-spec/blob/master/PURL-SPECIFICATION.rst). Components are designed such that they form a hierarchy from the most significant on the left to the least significant components on the right. 

Parsing a purl string into its components works from left to right. Some extra type-specific normalizations are required. For more information, see [How to parse a purl string in its components](https://github.com/package-url/purl-spec/blob/master/PURL-SPECIFICATION.rst#how-to-parse-a-purl-string-in-its-components).""" ;
    rdfs:domain software:Package ;
    rdfs:range xsd:anyURI ;
    ns0:term_status "Stable" .

software:packageVersion a owl:DatatypeProperty ;
    rdfs:comment "A packageVersion is useful for identification purposes and for indicating later changes of the package version." ;
    rdfs:domain software:Package ;
    rdfs:range xsd:string ;
    ns0:term_status "Stable" .

software:primaryPurpose a owl:ObjectProperty ;
    rdfs:comment "primaryPurpose provides information about the primary purpose of the software artifact." ;
    rdfs:domain software:SoftwareArtifact ;
    rdfs:range software:SoftwarePurpose ;
    ns0:term_status "Stable" .

software:sbomType a owl:ObjectProperty ;
    rdfs:comment """This field is a reasonable estimation of the type of SBOM created from a creator perspective.
It is intended to be used to give guidance on the elements that may be contained within it.
Aligning with the guidance produced in [Types of Software Bill of Material (SBOM) Documents](https://www.cisa.gov/sites/default/files/2023-04/sbom-types-document-508c.pdf).""" ;
    rdfs:domain software:Sbom ;
    rdfs:range software:SbomType ;
    ns0:term_status "Stable" .

software:snippetFromFile a owl:ObjectProperty ;
    rdfs:comment "The field identifies the file which contains the snippet." ;
    rdfs:domain software:Snippet ;
    rdfs:range software:File ;
    ns0:term_status "Stable" .

software:softwareLinkage a owl:ObjectProperty ;
    rdfs:comment "A softwareLinkage is TODO" ;
    rdfs:domain software:SoftwareDependencyRelationship ;
    rdfs:range software:SoftwareDependencyLinkType ;
    ns0:term_status "Stable" .

software:sourceInfo a owl:DatatypeProperty ;
    rdfs:comment """SourceInfo records any relevant background information or additional comments
about the origin of the package. For example, this field might include comments 
indicating whether the package was pulled from a source code management system 
or has been repackaged. The creator can provide additional information to describe
any anomalies or discoveries in the determination of the origin of the package.""" ;
    rdfs:domain software:Package ;
    rdfs:range xsd:string ;
    ns0:term_status "Stable" .

core:LifecycleScopedRelationship a owl:Class,
        sh:NodeShape ;
    rdfs:comment "TODO" ;
    rdfs:subClassOf core:Relationship ;
    ns0:term_status "Stable" ;
    sh:property [ sh:class core:LifecycleScopeType ;
            sh:maxCount 1 ;
            sh:name "scope" ;
            sh:path core:scope ] .

core:Tool a owl:Class,
        sh:NodeShape ;
    rdfs:comment "A Tool is an element of hardware and/or software utilized to carry out a particular function." ;
    rdfs:subClassOf core:Element ;
    ns0:term_status "Stable" .

core:contentType a owl:DatatypeProperty ;
    rdfs:comment "ContentType specifies the media type of an Element." ;
    rdfs:range core:MediaType ;
    ns0:term_status "Stable" ;
    sh:or ( [ rdfs:domain core:Annotation,
                    core:ExternalRef ] ) .

core:verifiedUsing a owl:ObjectProperty ;
    rdfs:comment "VerifiedUsing provides an IntegrityMethod with which the integrity of an Element can be asserted." ;
    rdfs:range core:IntegrityMethod ;
    ns0:term_status "Stable" ;
    sh:or ( [ rdfs:domain core:Element,
                    core:ExternalMap ] ) .

expandedlicensing:ListedLicense a owl:Class,
        sh:NodeShape ;
    rdfs:comment """A ListedLicense represents a License that is listed on the SPDX License List
at https://spdx.org/licenses.""" ;
    rdfs:subClassOf expandedlicensing:License ;
    ns0:term_status "Stable" ;
    sh:property [ sh:datatype xsd:string ;
            sh:maxCount 1 ;
            sh:name "listVersionAdded" ;
            sh:path expandedlicensing:listVersionAdded ],
        [ sh:datatype xsd:string ;
            sh:maxCount 1 ;
            sh:name "deprecatedVersion" ;
            sh:path expandedlicensing:deprecatedVersion ] .

expandedlicensing:ListedLicenseException a owl:Class,
        sh:NodeShape ;
    rdfs:comment """A ListedLicenseException represents an exception to a License (in other words,
an exception to a license condition or an additional permission beyond those
granted in a License) which is listed on the SPDX Exceptions List at
https://spdx.org/licenses/exceptions-index.html.""" ;
    rdfs:subClassOf expandedlicensing:LicenseAddition ;
    ns0:term_status "Stable" ;
    sh:property [ sh:datatype xsd:string ;
            sh:maxCount 1 ;
            sh:name "listVersionAdded" ;
            sh:path expandedlicensing:listVersionAdded ],
        [ sh:datatype xsd:string ;
            sh:maxCount 1 ;
            sh:name "deprecatedVersion" ;
            sh:path expandedlicensing:deprecatedVersion ] .

expandedlicensing:WithAdditionOperator a owl:Class,
        sh:NodeShape ;
    rdfs:comment """A WithAdditionOperator indicates that the designated License is subject to the
designated LicenseAddition, which might be a license exception on the SPDX
Exceptions List (ListedLicenseException) or may be other additional text
(CustomLicenseAddition). It is represented in the SPDX License Expression
Syntax by the `WITH` operator.""" ;
    rdfs:subClassOf simplelicensing:AnyLicenseInfo ;
    ns0:term_status "Stable" ;
    sh:property [ sh:class expandedlicensing:ExtendableLicense ;
            sh:maxCount 1 ;
            sh:minCount 1 ;
            sh:name "subjectLicense" ;
            sh:path expandedlicensing:subjectLicense ],
        [ sh:class expandedlicensing:LicenseAddition ;
            sh:maxCount 1 ;
            sh:minCount 1 ;
            sh:name "subjectAddition" ;
            sh:path expandedlicensing:subjectAddition ] .

expandedlicensing:deprecatedVersion a owl:DatatypeProperty ;
    rdfs:comment """A deprecatedVersion for a ListedLicense or ListedLicenseException on the SPDX
License List specifies which version release of the License List was the first
one in which it was marked as deprecated.""" ;
    rdfs:range xsd:string ;
    ns0:term_status "Stable" ;
    sh:or ( [ rdfs:domain expandedlicensing:ListedLicense,
                    expandedlicensing:ListedLicenseException ] ) .

expandedlicensing:licenseXml a owl:DatatypeProperty ;
    rdfs:comment """The license XML format is defined and used by the SPDX legal team.
See the XML fields defined at https://github.com/spdx/license-list-XML/blob/main/DOCS/xml-fields.md for a text description.
There is also an XML schema available at https://github.com/spdx/license-list-XML/blob/main/schema/ListedLicense.xsd.""" ;
    rdfs:range xsd:string ;
    ns0:term_status "Stable" ;
    sh:or ( [ rdfs:domain expandedlicensing:License,
                    expandedlicensing:LicenseAddition ] ) .

expandedlicensing:listVersionAdded a owl:DatatypeProperty ;
    rdfs:comment """A listVersionAdded for a ListedLicense or ListedLicenseException on the SPDX
License List specifies which version release of the License List was the first
one in which it was included.""" ;
    rdfs:range xsd:string ;
    ns0:term_status "Stable" ;
    sh:or ( [ rdfs:domain expandedlicensing:ListedLicense,
                    expandedlicensing:ListedLicenseException ] ) .

expandedlicensing:member a owl:ObjectProperty ;
    rdfs:comment """A member is a license expression participating in a conjunctive (of type
ConjunctiveLicenseSet) or a disjunctive (of type DisjunctiveLicenseSet)
license set.""" ;
    rdfs:range simplelicensing:AnyLicenseInfo ;
    ns0:term_status "Stable" ;
    sh:or ( [ rdfs:domain expandedlicensing:ConjunctiveLicenseSet,
                    expandedlicensing:DisjunctiveLicenseSet ] ) .

expandedlicensing:obsoletedBy a owl:DatatypeProperty ;
    rdfs:comment """An obsoletedBy value for a deprecated License or LicenseAddition specifies
the licenseId of the replacement License or LicenseAddition that is preferred
to be used in its place. It should use the same format as specified for a
licenseId.

The License's or LicenseAddition's comment value may include more information
about the reason why the licenseId specified in the obsoletedBy value is
preferred.""" ;
    rdfs:range xsd:string ;
    ns0:term_status "Stable" ;
    sh:or ( [ rdfs:domain expandedlicensing:License,
                    expandedlicensing:LicenseAddition ] ) .

expandedlicensing:subjectLicense a owl:ObjectProperty ;
    rdfs:comment """A subjectLicense is a License which is subject to either an 'or later' effect
(OrLaterOperator) or a 'with additional text' effect (WithAdditionOperator).""" ;
    rdfs:range expandedlicensing:License ;
    ns0:term_status "Stable" ;
    sh:or ( [ rdfs:domain expandedlicensing:OrLaterOperator,
                    expandedlicensing:WithAdditionOperator ] ) .

security:CvssV2VulnAssessmentRelationship a owl:Class,
        sh:NodeShape ;
    rdfs:comment """A CvssV2VulnAssessmentRelationship relationship describes the determined score and vector of a vulnerability using version 2.0 of the Common Vulnerability Scoring System (CVSS) as defined at [https://www.first.org/cvss/v2/guide](https://www.first.org/cvss/v2/guide). It is intended to communicate the results of using a CVSS calculator.

**Constraints**

- The relationship type must be set to `hasAssessmentFor`.

**Syntax**

```json
{
  "@type": "CvssV2VulnAssessmentRelationship",
  "@id": "urn:spdx.dev:cvssv2-cve-2020-28498",
  "relationshipType": "hasAssessmentFor",
  "score": 4.3,
  "vectorString": "(AV:N/AC:M/Au:N/C:P/I:N/A:N)",
  "from": "urn:spdx.dev:vuln-cve-2020-28498",
  "to": ["urn:product-acme-application-1.3"],
  "assessedElement": "urn:npm-elliptic-6.5.2",
  "externalRefs": [
    {
      "@type": "ExternalRef",
      "externalRefType": "securityAdvisory",
      "locator": "https://nvd.nist.gov/vuln/detail/CVE-2020-28498"
    },
    {
      "@type": "ExternalRef",
      "externalRefType": "securityAdvisory",
      "locator": "https://snyk.io/vuln/SNYK-JS-ELLIPTIC-1064899"
    },
    {
      "@type": "ExternalRef",
      "externalRefType": "securityFix",
      "locator": "https://github.com/indutny/elliptic/commit/441b742"
    }
  ],
  "suppliedBy": ["urn:spdx.dev:agent-my-security-vendor"],
  "publishedTime": "2023-05-06T10:06:13Z"
},
{
  "@type": "Relationship",
  "@id": "urn:spdx.dev:vulnAgentRel-1",  
  "relationshipType": "publishedBy",  
  "from": "urn:spdx.dev:cvssv2-cve-2020-28498",
  "to": ["urn:spdx.dev:agent-snyk"],
  "startTime": "2021-03-08T16:06:50Z"
}
```""" ;
    rdfs:subClassOf security:VulnAssessmentRelationship ;
    ns0:term_status "Stable" ;
    sh:property [ sh:datatype xsd:string ;
            sh:maxCount 1 ;
            sh:minCount 1 ;
            sh:name "vectorString" ;
            sh:path security:vectorString ],
        [ sh:datatype xsd:decimal ;
            sh:maxCount 1 ;
            sh:minCount 1 ;
            sh:name "score" ;
            sh:path security:score ] .

security:VexAffectedVulnAssessmentRelationship a owl:Class,
        sh:NodeShape ;
    rdfs:comment """VexAffectedVulnAssessmentRelationship connects a vulnerability and a number
of elements. The relationship marks these elements as products affected by the
vulnerability. This relationship corresponds to the VEX affected status.

**Constraints**

When linking elements using a VexAffectedVulnAssessmentRelationship, the
following requirements must be observed:

- Elements linked with a VulnVexAffectedAssessmentRelationship are constrained
to the affects relationship type.

**Syntax**

```json
{
  "@type": "VexAffectedVulnAssessmentRelationship",
  "@id": "urn:spdx.dev:vex-affected-1",
  "relationshipType": "affects",
  "from": "urn:spdx.dev:vuln-cve-2020-28498",
  "to": ["urn:product-acme-application-1.3"],
  "assessedElement": "urn:npm-elliptic-6.5.2",
  "actionStatement": "Upgrade to version 1.4 of ACME application.",
  "suppliedBy": ["urn:spdx.dev:agent-jane-doe"],
  "publishedTime": "2021-03-09T11:04:53Z"
}
```""" ;
    rdfs:subClassOf security:VexVulnAssessmentRelationship ;
    ns0:term_status "Stable" ;
    sh:property [ sh:datatype core:DateTime ;
            sh:name "actionStatementTime" ;
            sh:path security:actionStatementTime ],
        [ sh:datatype xsd:string ;
            sh:maxCount 1 ;
            sh:name "actionStatement" ;
            sh:path security:actionStatement ] .

security:modifiedTime a owl:DatatypeProperty ;
    rdfs:comment "Specifies a time when a vulnerability assessment was last modified." ;
    rdfs:range core:DateTime ;
    ns0:term_status "Stable" ;
    sh:or ( [ rdfs:domain security:VulnAssessmentRelationship,
                    security:Vulnerability ] ) .

security:severity a owl:DatatypeProperty ;
    rdfs:comment "The severity field provides a human readable string of the resulting numerical CVSS score." ;
    rdfs:range security:CvssSeverityType ;
    ns0:term_status "Stable" ;
    sh:or ( [ rdfs:domain security:CvssV3VulnAssessmentRelationship,
                    security:CvssV4VulnAssessmentRelationship ] ) .

security:withdrawnTime a owl:DatatypeProperty ;
    rdfs:comment "Specified the time and date when a vulnerability was withdrawn." ;
    rdfs:range core:DateTime ;
    ns0:term_status "Stable" ;
    sh:or ( [ rdfs:domain security:VulnAssessmentRelationship,
                    security:Vulnerability ] ) .

simplelicensing:licenseText a owl:DatatypeProperty ;
    rdfs:comment """A licenseText contains the plain text of the License or Addition,
without templating or other similar markup.

Users of the licenseText for a License can apply the SPDX Matching Guidelines
when comparing it to another text for matching purposes.""" ;
    rdfs:domain simplelicensing:SimpleLicensingText ;
    rdfs:range xsd:string ;
    ns0:term_status "Stable" .

software:SoftwareDependencyRelationship a owl:Class,
        sh:NodeShape ;
    rdfs:comment "TODO" ;
    rdfs:subClassOf core:LifecycleScopedRelationship ;
    ns0:term_status "Stable" ;
    sh:property [ sh:class software:SoftwareDependencyLinkType ;
            sh:maxCount 1 ;
            sh:name "softwareLinkage" ;
            sh:path software:softwareLinkage ],
        [ sh:class software:DependencyConditionalityType ;
            sh:maxCount 1 ;
            sh:name "conditionality" ;
            sh:path software:conditionality ] .

core:Bundle a owl:Class,
        sh:NodeShape ;
    rdfs:comment "A bundle is a collection of Elements that have a shared context." ;
    rdfs:subClassOf core:ElementCollection ;
    ns0:term_status "Stable" ;
    sh:property [ sh:datatype xsd:string ;
            sh:maxCount 1 ;
            sh:name "context" ;
            sh:path core:context ] .

expandedlicensing:ExtendableLicense a owl:Class,
        sh:NodeShape ;
    rdfs:comment "The WithAdditionOperator can have a License or an OrLaterOperator as the license property value.  This class is used for the value." ;
    rdfs:subClassOf simplelicensing:AnyLicenseInfo ;
    ns0:term_status "Stable" .

security:CvssV3VulnAssessmentRelationship a owl:Class,
        sh:NodeShape ;
    rdfs:comment """A CvssV3VulnAssessmentRelationship relationship describes the determined score,
severity, and vector of a vulnerability using version [3.0](https://www.first.org/cvss/v3.0/specification-document) or [3.1](https://www.first.org/cvss/v3.1/specification-document) of the Common
Vulnerability Scoring System (CVSS). It is intended to communicate the results of using a CVSS calculator.

**Constraints**

- The value of severity must be one of 'NONE', 'LOW', 'MEDIUM', 'HIGH' or 'CRITICAL'.
- The relationship type must be set to `hasAssessmentFor`.

**Syntax**

```json
{
  "@type": "CvssV3VulnAssessmentRelationship",
  "@id": "urn:spdx.dev:cvssv3-cve-2020-28498",
  "relationshipType": "hasAssessmentFor",
  "score": 6.8,
  "severity": "MEDIUM",
  "vectorString": "CVSS:3.1/AV:N/AC:H/PR:N/UI:N/S:C/C:H/I:N/A:N",
  "from": "urn:spdx.dev:vuln-cve-2020-28498",
  "to": ["urn:product-acme-application-1.3"],
  "assessedElement": "urn:npm-elliptic-6.5.2",
  "externalRefs": [
    {
      "@type": "ExternalRef",
      "externalRefType": "securityAdvisory",
      "locator": "https://nvd.nist.gov/vuln/detail/CVE-2020-28498"
    },
    {
      "@type": "ExternalRef",
      "externalRefType": "securityAdvisory",
      "locator": "https://snyk.io/vuln/SNYK-JS-ELLIPTIC-1064899"
    },
    {
      "@type": "ExternalRef",
      "externalRefType": "securityFix",
      "locator": "https://github.com/indutny/elliptic/commit/441b742"
    }
  ],
  "suppliedBy": ["urn:spdx.dev:agent-my-security-vendor"],
  "publishedTime": "2023-05-06T10:06:13Z"
},
{
  "@type": "Relationship",
  "@id": "urn:spdx.dev:vulnAgentRel-1",
  "relationshipType": "publishedBy",
  "from": "urn:spdx.dev:cvssv3-cve-2020-28498",
  "to": "urn:spdx.dev:agent-snyk",
  "startTime": "2021-03-08T16:06:50Z"
}
```""" ;
    rdfs:subClassOf security:VulnAssessmentRelationship ;
    ns0:term_status "Stable" ;
    sh:property [ sh:datatype xsd:decimal ;
            sh:maxCount 1 ;
            sh:minCount 1 ;
            sh:name "score" ;
            sh:path security:score ],
        [ sh:datatype xsd:string ;
            sh:maxCount 1 ;
            sh:minCount 1 ;
            sh:name "vectorString" ;
            sh:path security:vectorString ],
        [ sh:class security:CvssSeverityType ;
            sh:maxCount 1 ;
            sh:minCount 1 ;
            sh:name "severity" ;
            sh:path security:severity ] .

security:CvssV4VulnAssessmentRelationship a owl:Class,
        sh:NodeShape ;
    rdfs:comment """A CvssV4VulnAssessmentRelationship relationship describes the determined score, severity, and vector of a vulnerability using version 4 of the Common Vulnerability Scoring System (CVSS) as defined on [https://www.first.org/cvss/v4.0/specification-document](https://www.first.org/cvss/v4.0/specification-document). It is intented to communicate the results of using a CVSS calculator.

**Constraints**

- The value of severity must be one of 'NONE', 'LOW', 'MEDIUM', 'HIGH' or 'CRITICAL'.
- The relationship type must be set to hasAssessmentFor.

**Syntax**

```json
{
  "@type": "CvssV4VulnAssessmentRelationship",
  "@id": "urn:spdx.dev:cvssv4-cve-2021-44228",
  "relationshipType": "hasAssessmentFor",
  "severity": "MEDIUM",
  "score": 10.0,
  "vectorString": "CVSS:4.0/AV:N/AC:L/AT:N/AR:N/UI:N/VCH/VI:H/VA:H/SC:H/SI:H/SA:H/E:A",
  "from": "urn:spdx.dev:vuln-cve-2021-44228",
  "to": ["urn:product-acme-application-1.3"],
  "assessedElement": "urn:apache-log4j-2.14.1",
  "externalRefs": [
    {
      "@type": "ExternalRef",
      "externalRefType": "securityAdvisory",
      "locator": "https://nvd.nist.gov/vuln/detail/CVE-2021-44228"
    },
    {
      "@type": "ExternalRef",
      "externalRefType": "securityAdvisory",
      "locator": "https://logging.apache.org/log4j/2.x/security.html"
    },
    {
      "@type": "ExternalRef",
      "externalRefType": "securityOther",
      "locator": "    https://www.first.org/cvss/v4.0/examples#Apache-log4j-JNDI-Command-Execution-log4shell-Vulnerability-CVE-2021-44228"
    },
  ],
  "suppliedBy": ["urn:spdx.dev:agent-my-security-vendor"],
  "publishedTime": "2023-10-05T23:09:13Z"
},
{
  "@type": "Relationship",
  "@id": "urn:spdx.dev:vulnAgentRel-1",
  "relationshipType": "publishedBy",
  "from": "urn:spdx.dev:cvssv4-cve-2021-44228",
  "to": "urn:spdx.dev:agent-apache.org",
  "startTime": "2021-12-11T18:39:00Z"
}
```""" ;
    rdfs:subClassOf security:VulnAssessmentRelationship ;
    ns0:term_status "Stable" ;
    sh:property [ sh:class security:CvssSeverityType ;
            sh:maxCount 1 ;
            sh:minCount 1 ;
            sh:name "severity" ;
            sh:path security:severity ],
        [ sh:datatype xsd:string ;
            sh:maxCount 1 ;
            sh:minCount 1 ;
            sh:name "vectorString" ;
            sh:path security:vectorString ],
        [ sh:datatype xsd:decimal ;
            sh:maxCount 1 ;
            sh:minCount 1 ;
            sh:name "score" ;
            sh:path security:score ] .

security:EpssVulnAssessmentRelationship a owl:Class,
        sh:NodeShape ;
    rdfs:comment """An EpssVulnAssessmentRelationship relationship describes the likelihood or probability that a vulnerability will be exploited in the wild using the Exploit Prediction Scoring System (EPSS) as defined at [https://www.first.org/epss/model](https://www.first.org/epss/model).

**Constraints**

- The relationship type must be set to hasAssessmentFor.
- The probability must be between 0 and 1.
- The percentile must be between 0 and 1.

**Syntax**

```json
{
  "@type": "EpssVulnAssessmentRelationship",
  "@id": "urn:spdx.dev:epss-CVE-2020-28498",
  "relationshipType": "hasAssessmentFor",
  "probability": 0.00105,
  "percentile": 0.42356,
  "from": "urn:spdx.dev:vuln-cve-2020-28498",
  "to": ["urn:product-acme-application-1.3"],
  "suppliedBy": ["urn:spdx.dev:agent-jane-doe"],
  "publishedTime": "2023-10-05T00:00:30Z"
}
```""" ;
    rdfs:subClassOf security:VulnAssessmentRelationship ;
    ns0:term_status "Stable" ;
    sh:property [ sh:datatype core:DateTime ;
            sh:maxCount 1 ;
            sh:minCount 1 ;
            sh:name "publishedTime" ;
            sh:path security:publishedTime ],
        [ sh:datatype xsd:decimal ;
            sh:maxCount 1 ;
            sh:minCount 1 ;
            sh:name "probability" ;
            sh:path security:probability ],
        [ sh:datatype xsd:decimal ;
            sh:maxCount 1 ;
            sh:minCount 1 ;
            sh:name "percentile" ;
            sh:path security:percentile ] .

security:ExploitCatalogVulnAssessmentRelationship a owl:Class,
        sh:NodeShape ;
    rdfs:comment """An ExploitCatalogVulnAssessmentRelationship describes if a vulnerability is
listed in any exploit catalog such as the CISA Known Exploited Vulnerabilities
Catalog (KEV) 
[https://www.cisa.gov/known-exploited-vulnerabilities-catalog](https://www.cisa.gov/known-exploited-vulnerabilities-catalog).

**Constraints**

- The relationship type must be set to hasAssessmentFor.

**Syntax**

```json
{
  "@type": "ExploitCatalogVulnAssessmentRelationship",
  "@id": "urn:spdx.dev:exploit-catalog-1",
  "relationshipType": "hasAssessmentFor",
  "catalogType": "kev",
  "locator": "https://www.cisa.gov/known-exploited-vulnerabilities-catalog",
  "exploited": "true",
  "from": "urn:spdx.dev:vuln-cve-2023-2136",
  "to": ["urn:product-google-chrome-112.0.5615.136"],
  "suppliedBy": ["urn:spdx.dev:agent-jane-doe"],
  "publishedTime": "2021-03-09T11:04:53Z"
}
```""" ;
    rdfs:subClassOf security:VulnAssessmentRelationship ;
    ns0:term_status "Stable" ;
    sh:property [ sh:datatype xsd:boolean ;
            sh:maxCount 1 ;
            sh:minCount 1 ;
            sh:name "exploited" ;
            sh:path security:exploited ],
        [ sh:datatype xsd:anyURI ;
            sh:maxCount 1 ;
            sh:minCount 1 ;
            sh:name "locator" ;
            sh:path security:locator ],
        [ sh:class security:ExploitCatalogType ;
            sh:maxCount 1 ;
            sh:minCount 1 ;
            sh:name "catalogType" ;
            sh:path security:catalogType ] .

security:VexNotAffectedVulnAssessmentRelationship a owl:Class,
        sh:NodeShape ;
    rdfs:comment """VexNotAffectedVulnAssessmentRelationship connects a vulnerability and a number
of elements designating them as products not affected by the vulnerability.
This relationship corresponds to the VEX not_affected status.

**Constraints**

When linking elements using a VexNotVulnAffectedAssessmentRelationship, the
following requirements must be observed:

* Relating elements with a VexNotAffectedVulnAssessmentRelationship is restricted
to the doesNotAffect relationship type.
* The from: end of the relationship must be a /Security/Vulnerability classed
element.
* Both impactStatement and justificationType properties have a cardinality of
0..1 making them optional. Nevertheless, to produce a valid VEX not_affected
statement, one of them MUST be defined. This is specified in the Minimum Elements
for VEX.

**Syntax**

```json
{
  "@type": "VexNotAffectedVulnAssessmentRelationship",
  "@id": "urn:spdx.dev:vex-not-affected-1",
  "relationshipType": "doesNotAffect",
  "from": "urn:spdx.dev:vuln-cve-2020-28498",
  "to": ["urn:product-acme-application-1.3"],
  "assessedElement": "urn:npm-elliptic-6.5.2",
  "justificationType": "componentNotPresent",
  "impactStatement": "Not using this vulnerable part of this library.",
  "suppliedBy": ["urn:spdx.dev:agent-jane-doe"],
  "publishedTime": "2021-03-09T11:04:53Z"
}
```""" ;
    rdfs:subClassOf security:VexVulnAssessmentRelationship ;
    ns0:term_status "Stable" ;
    sh:property [ sh:class security:VexJustificationType ;
            sh:maxCount 1 ;
            sh:name "justificationType" ;
            sh:path security:justificationType ],
        [ sh:datatype xsd:string ;
            sh:maxCount 1 ;
            sh:name "impactStatement" ;
            sh:path security:impactStatement ],
        [ sh:datatype core:DateTime ;
            sh:maxCount 1 ;
            sh:name "impactStatementTime" ;
            sh:path security:impactStatementTime ] .

security:Vulnerability a owl:Class,
        sh:NodeShape ;
    rdfs:comment """Specifies a vulnerability and its associated information.

**Syntax**

```json
{
  "@type": "Vulnerability",
  "@id": "urn:spdx.dev:vuln-1",
  "summary": "Use of a Broken or Risky Cryptographic Algorithm",
  "description": "The npm package `elliptic` before version 6.5.4 are vulnerable to Cryptographic Issues via the secp256k1 implementation in elliptic/ec/key.js. There is no check to confirm that the public key point passed into the derive function actually exists on the secp256k1 curve. This results in the potential for the private key used in this implementation to be revealed after a number of ECDH operations are performed.",      
  "modified": "2021-03-08T16:02:43Z",
  "published": "2021-03-08T16:06:50Z",
  "externalIdentifiers": [
    {
      "@type": "ExternalIdentifier",
      "externalIdentifierType": "cve",
      "identifier": "CVE-2020-2849",
      "identifierLocator": [
        "https://cve.mitre.org/cgi-bin/cvename.cgi?name=CVE-2020-28498",
        "https://www.cve.org/CVERecord?id=CVE-2020-28498"
      ],
      "issuingAuthority": "urn:spdx.dev:agent-cve.org"
    },
    {
      "type": "ExternalIdentifier",
      "externalIdentifierType": "securityOther",
      "identifier": "GHSA-r9p9-mrjm-926w",
      "identifierLocator": "https://github.com/advisories/GHSA-r9p9-mrjm-926w"
    },
    {
      "type": "ExternalIdentifier",
      "externalIdentifierType": "securityOther",
      "identifier": "SNYK-JS-ELLIPTIC-1064899",
      "identifierLocator": "https://security.snyk.io/vuln/SNYK-JS-ELLIPTIC-1064899"
    }
  ],
  "externalRefs": [
    {
        "@type": "ExternalRef",
        "externalRefType": "securityAdvisory",
        "locator": "https://nvd.nist.gov/vuln/detail/CVE-2020-28498"
    },
    {
      "@type": "ExternalRef",
      "externalRefType": "securityAdvisory",
      "locator": "https://ubuntu.com/security/CVE-2020-28498"
    },
    {
      "@type": "ExternalRef",
      "externalRefType": "securityOther",
      "locator": "https://github.com/indutny/elliptic/pull/244/commits"
    },
    {
      "@type": "ExternalRef",
      "externalRefType": "securityOther",
      "locator": "https://github.com/christianlundkvist/blog/blob/master/2020_05_26_secp256k1_twist_attacks/secp256k1_twist_attacks.md"
    }
  ]
},
{
  "@type": "Relationship",
  "@id": "urn:spdx.dev:vulnRelationship-1",
  "relationshipType": "hasAssociatedVulnerability",
  "from": "urn:npm-elliptic-6.5.2",
  "to": ["urn:spdx.dev:vuln-1"],
  "startTime": "2021-03-08T16:06:50Z"
},
{
  "@type": "Relationship",
  "@id": "urn:spdx.dev:vulnAgentRel-1",  
  "relationshipType": "publishedBy",  
  "from": "urn:spdx.dev:vuln-1",
  "to": ["urn:spdx.dev:agent-snyk"],
  "startTime": "2021-03-08T16:06:50Z"
}
```""" ;
    rdfs:subClassOf core:Artifact ;
    ns0:term_status "Stable" ;
    sh:property [ sh:datatype core:DateTime ;
            sh:maxCount 1 ;
            sh:name "withdrawnTime" ;
            sh:path security:withdrawnTime ],
        [ sh:datatype core:DateTime ;
            sh:maxCount 1 ;
            sh:name "publishedTime" ;
            sh:path security:publishedTime ],
        [ sh:datatype core:DateTime ;
            sh:maxCount 1 ;
            sh:name "modifiedTime" ;
            sh:path security:modifiedTime ] .

security:publishedTime a owl:DatatypeProperty ;
    rdfs:comment "Specifies the time when a vulnerability was first published." ;
    rdfs:range core:DateTime ;
    ns0:term_status "Stable" ;
    sh:or ( [ rdfs:domain security:EpssVulnAssessmentRelationship,
                    security:VulnAssessmentRelationship,
                    security:Vulnerability ] ) .

security:score a owl:DatatypeProperty ;
    rdfs:comment """The score provides information on the severity of a vulnerability per the
Common Vulnerability Scoring System as defined on [https://www.first.org/cvss](https://www.first.org/cvss/).""" ;
    rdfs:range xsd:string ;
    ns0:term_status "Stable" ;
    sh:or ( [ rdfs:domain security:CvssV2VulnAssessmentRelationship,
                    security:CvssV3VulnAssessmentRelationship,
                    security:CvssV4VulnAssessmentRelationship ] ) .

security:vectorString a owl:DatatypeProperty ;
    rdfs:comment """Specifies any combination of the CVSS Base, Temporal, Threat, Environmental, and/or Supplemental vector string values for a vulnerability. Supports vectorStrings specified in all CVSS versions.

**Constraints**

String values for the vectorString range must only include the abbreviated form of metric names specified in CVSS specifications, e.g. [https://www.first.org/cvss/v4.0/specification-document#Vector-String](https://www.first.org/cvss/v4.0/specification-document#Vector-String)""" ;
    rdfs:range xsd:string ;
    ns0:term_status "Stable" ;
    sh:or ( [ rdfs:domain security:CvssV2VulnAssessmentRelationship,
                    security:CvssV3VulnAssessmentRelationship,
                    security:CvssV4VulnAssessmentRelationship ] ) .

simplelicensing:LicenseExpression a owl:Class,
        sh:NodeShape ;
    rdfs:comment """Often a single license can be used to represent the licensing terms of a source code or binary file, but there are situations where a single license identifier is not sufficient. A common example is when software is offered under a choice of one or more licenses (e.g., GPL-2.0-only OR BSD-3-Clause). Another example is when a set of licenses is needed to represent a binary program constructed by compiling and linking two (or more) different source files each governed by different licenses (e.g., LGPL-2.1-only AND BSD-3-Clause).

SPDX License Expressions provide a way for one to construct expressions that more accurately represent the licensing terms typically found in open source software source code. A license expression could be a single license identifier found on the SPDX License List; a user defined license reference denoted by the LicenseRef-idString; a license identifier combined with an SPDX exception; or some combination of license identifiers, license references and exceptions constructed using a small set of defined operators (e.g., AND, OR, WITH and +). We provide the definition of what constitutes a valid an SPDX License Expression in this section.""" ;
    rdfs:subClassOf simplelicensing:AnyLicenseInfo ;
    ns0:term_status "Stable" ;
    sh:property [ sh:datatype core:SemVer ;
            sh:maxCount 1 ;
            sh:name "licenseListVersion" ;
            sh:path simplelicensing:licenseListVersion ],
        [ sh:class core:DictionaryEntry ;
            sh:name "customIdToUri" ;
            sh:path simplelicensing:customIdToUri ],
        [ sh:datatype xsd:string ;
            sh:maxCount 1 ;
            sh:minCount 1 ;
            sh:name "licenseExpression" ;
            sh:path simplelicensing:licenseExpression ] .

software:File a owl:Class,
        sh:NodeShape ;
    rdfs:comment """Refers to any object that stores content on a computer.
The type of content can optionally be provided in the contentType property.
External property restriction on /Core/Element/name: minCount: 1""" ;
    rdfs:subClassOf software:SoftwareArtifact ;
    ns0:term_status "Stable" ;
    sh:property [ sh:datatype core:MediaType ;
            sh:maxCount 1 ;
            sh:name "contentType" ;
            sh:path software:contentType ] .

software:Snippet a owl:Class,
        sh:NodeShape ;
    rdfs:comment """A Snippet describes a certain part of a file and can be used when the file is known to have some content
that has been included from another original source. Snippets are useful for denoting when part of a file
may have been originally created under another license or copied from a place with a known vulnerability.""" ;
    rdfs:subClassOf software:SoftwareArtifact ;
    ns0:term_status "Stable" ;
    sh:property [ sh:class core:PositiveIntegerRange ;
            sh:maxCount 1 ;
            sh:name "byteRange" ;
            sh:path software:byteRange ],
        [ sh:class core:PositiveIntegerRange ;
            sh:maxCount 1 ;
            sh:name "lineRange" ;
            sh:path software:lineRange ],
        [ sh:class software:File ;
            sh:maxCount 1 ;
            sh:minCount 1 ;
            sh:name "snippetFromFile" ;
            sh:path software:snippetFromFile ] .

core:Annotation a owl:Class,
        sh:NodeShape ;
    rdfs:comment "An Annotation is an assertion made in relation to one or more elements." ;
    rdfs:subClassOf core:Element ;
    ns0:term_status "Stable" ;
    sh:property [ sh:datatype xsd:string ;
            sh:maxCount 1 ;
            sh:name "statement" ;
            sh:path core:statement ],
        [ sh:class core:Element ;
            sh:maxCount 1 ;
            sh:minCount 1 ;
            sh:name "subject" ;
            sh:path core:subject ],
        [ sh:class core:AnnotationType ;
            sh:maxCount 1 ;
            sh:minCount 1 ;
            sh:name "annotationType" ;
            sh:path core:annotationType ],
        [ sh:datatype core:MediaType ;
            sh:name "contentType" ;
            sh:path core:contentType ] .

core:AnnotationType a owl:Class ;
    rdfs:comment "AnnotationType specifies the type of an annotation." ;
    owl:oneOf ( <https://spdx.org/rdf/v3/Core/AnnotationType/other> <https://spdx.org/rdf/v3/Core/AnnotationType/review> ) ;
    ns0:term_status "Stable" .

core:Hash a owl:Class,
        sh:NodeShape ;
    rdfs:comment """A hash is a grouping of characteristics unique to the result
of applying a mathematical algorithm
that maps data of arbitrary size to a bit string (the hash)
and is a one-way function, that is,
a function which is practically infeasible to invert.
This is commonly used for integrity checking of data.""" ;
    rdfs:subClassOf core:IntegrityMethod ;
    ns0:term_status "Stable" ;
    sh:property [ sh:class core:HashAlgorithm ;
            sh:maxCount 1 ;
            sh:minCount 1 ;
            sh:name "algorithm" ;
            sh:path core:algorithm ],
        [ sh:datatype xsd:string ;
            sh:maxCount 1 ;
            sh:minCount 1 ;
            sh:name "hashValue" ;
            sh:path core:hashValue ] .

security:ExploitCatalogType a owl:Class ;
    rdfs:comment "ExploitCatalogType specifies the type of exploit catalog that a vulnerability is listed in." ;
    owl:oneOf ( <https://spdx.org/rdf/v3/Security/ExploitCatalogType/other> <https://spdx.org/rdf/v3/Security/ExploitCatalogType/kev> ) ;
    ns0:term_status "Stable" .

core:ElementCollection a owl:Class,
        sh:NodeShape ;
    rdfs:comment """An ElementCollection is a collection of Elements, not necessarily with unifying context.

Note that all ElementCollections must conform to the core profile even if the core profile is no specified in the profileConformance property.
If the profileConformance property is not provided, core is to be assumed as the default.

**Constraints**
If the ElementCollection has at least 1 element, it must also have at least 1 rootElement""" ;
    rdfs:subClassOf core:Element ;
    ns0:term_status "Stable" ;
    sh:property [ sh:class core:Element ;
            sh:name "rootElement" ;
            sh:path core:rootElement ],
        [ sh:class core:ProfileIdentifierType ;
            sh:name "profileConformance" ;
            sh:path core:profileConformance ],
        [ sh:class core:Element ;
            sh:name "element" ;
            sh:path core:element ],
        [ sh:class core:ExternalMap ;
            sh:name "imports" ;
            sh:path core:imports ] .

core:IntegrityMethod a owl:Class,
        sh:NodeShape ;
    rdfs:comment """An IntegrityMethod provides an independently reproducible mechanism that permits verification
of a specific Element that correlates to the data in this SPDX document. This identifier enables
a recipient to determine if anything in the original Element has been changed and eliminates
confusion over which version or modification of a specific Element is referenced.""" ;
    ns0:term_status "Stable" ;
    sh:property [ sh:datatype xsd:string ;
            sh:maxCount 1 ;
            sh:name "comment" ;
            sh:path core:comment ] .

core:RelationshipCompleteness a owl:Class ;
    rdfs:comment "RelationshipCompleteness indicates whether the provided relationship is known to be complete, known to be incomplete, or if no assertion is made by the relationship creator." ;
    owl:oneOf ( <https://spdx.org/rdf/v3/Core/RelationshipCompleteness/complete> <https://spdx.org/rdf/v3/Core/RelationshipCompleteness/noAssertion> <https://spdx.org/rdf/v3/Core/RelationshipCompleteness/incomplete> ) ;
    ns0:term_status "Stable" .

core:comment a owl:DatatypeProperty ;
    rdfs:comment """A comment is an optional field for creators of the Element to provide comments
to the readers/reviewers of the document.""" ;
    rdfs:range xsd:string ;
    ns0:term_status "Stable" ;
    sh:or ( [ rdfs:domain core:CreationInfo,
                    core:Element,
                    core:ExternalIdentifier,
                    core:ExternalRef,
                    core:IntegrityMethod ] ) .

ai:SafetyRiskAssessmentType a owl:Class ;
    rdfs:comment """Lists the different safety risk type values that can be used to describe the safety risk of AI software
according to [Article 20 of Regulation 765/2008/EC](https://ec.europa.eu/docsroom/documents/17107/attachments/1/translations/en/renditions/pdf).""" ;
    owl:oneOf ( <https://spdx.org/rdf/v3/AI/SafetyRiskAssessmentType/low> <https://spdx.org/rdf/v3/AI/SafetyRiskAssessmentType/high> <https://spdx.org/rdf/v3/AI/SafetyRiskAssessmentType/medium> <https://spdx.org/rdf/v3/AI/SafetyRiskAssessmentType/serious> ) ;
    ns0:term_status "Stable" .

core:ExternalMap a owl:Class,
        sh:NodeShape ;
    rdfs:comment """An External Map is a map of Element identifiers that are used within a Document
but defined external to that Document.
The external map provides details about the externally-defined Element
such as its provenance, where to retrieve it, and how to verify its integrity.""" ;
    rdfs:subClassOf owl:Thing ;
    ns0:term_status "Stable" ;
    sh:property [ sh:datatype xsd:anyURI ;
            sh:maxCount 1 ;
            sh:name "locationHint" ;
            sh:path core:locationHint ],
        [ sh:datatype xsd:anyURI ;
            sh:maxCount 1 ;
            sh:minCount 1 ;
            sh:name "externalSpdxId" ;
            sh:path core:externalSpdxId ],
        [ sh:class core:Artifact ;
            sh:maxCount 1 ;
            sh:name "definingDocument" ;
            sh:path core:definingDocument ],
        [ sh:class core:IntegrityMethod ;
            sh:name "verifiedUsing" ;
            sh:path core:verifiedUsing ] .

core:ExternalRef a owl:Class,
        sh:NodeShape ;
    rdfs:comment """An External Reference points to a resource outside the scope of the SPDX-3.0 content
that provides additional characteristics of an Element.""" ;
    rdfs:subClassOf owl:Thing ;
    ns0:term_status "Stable" ;
    sh:property [ sh:datatype xsd:string ;
            sh:name "locator" ;
            sh:path core:locator ],
        [ sh:datatype core:MediaType ;
            sh:maxCount 1 ;
            sh:name "contentType" ;
            sh:path core:contentType ],
        [ sh:datatype xsd:string ;
            sh:maxCount 1 ;
            sh:name "comment" ;
            sh:path core:comment ],
        [ sh:class core:ExternalRefType ;
            sh:maxCount 1 ;
            sh:name "externalRefType" ;
            sh:path core:externalRefType ] .

core:PositiveIntegerRange a owl:Class,
        sh:NodeShape ;
    rdfs:comment """PositiveIntegerRange is a tuple of two positive integers that define a range.
"begin" must be less than or equal to "end".""" ;
    rdfs:subClassOf owl:Thing ;
    ns0:term_status "Stable" ;
    sh:property [ sh:datatype xsd:positiveInteger ;
            sh:maxCount 1 ;
            sh:minCount 1 ;
            sh:name "end" ;
            sh:path core:end ],
        [ sh:datatype xsd:positiveInteger ;
            sh:maxCount 1 ;
            sh:minCount 1 ;
            sh:name "begin" ;
            sh:path core:begin ] .

dataset:ConfidentialityLevelType a owl:Class ;
    rdfs:comment "Describes the different confidentiality levels as given by the [Traffic Light Protocol](https://en.wikipedia.org/wiki/Traffic_Light_Protocol)." ;
    owl:oneOf ( <https://spdx.org/rdf/v3/Dataset/ConfidentialityLevelType/clear> <https://spdx.org/rdf/v3/Dataset/ConfidentialityLevelType/green> <https://spdx.org/rdf/v3/Dataset/ConfidentialityLevelType/red> <https://spdx.org/rdf/v3/Dataset/ConfidentialityLevelType/amber> ) ;
    ns0:term_status "Stable" .

security:SsvcDecisionType a owl:Class ;
    rdfs:comment "SsvcDecisionType specifies the type of decision that's been made according to the Stakeholder-Specific Vulnerability Categorization (SSVC)  system [https://www.cisa.gov/stakeholder-specific-vulnerability-categorization-ssvc](https://www.cisa.gov/stakeholder-specific-vulnerability-categorization-ssvc)" ;
    owl:oneOf ( <https://spdx.org/rdf/v3/Security/SsvcDecisionType/trackStar> <https://spdx.org/rdf/v3/Security/SsvcDecisionType/track> <https://spdx.org/rdf/v3/Security/SsvcDecisionType/attend> <https://spdx.org/rdf/v3/Security/SsvcDecisionType/act> ) ;
    ns0:term_status "Stable" .

security:VexVulnAssessmentRelationship a owl:Class,
        sh:NodeShape ;
    rdfs:comment """VexVulnAssessmentRelationship is an abstract subclass that defined the common
properties shared by all the SPDX-VEX status relationships. 

**Constraints**

When linking elements using a VexVulnAssessmentRelationship, the following
requirements must be observed:

- The from: end must be a /Security/Vulnerability classed element
- The to: end must point to elements representing the VEX _products_. To
specify a different element where the vulnerability was detected, the VEX
relationship can optionally specify _subcomponents_ using the assessedElement
property.

VEX inherits information from the document level down to its statements. When a
statement is missing information it can be completed by reading the equivalent 
field from the containing document. For example, if a VEX relationship is
missing data in its createdBy property, tools must consider the entity
listed in the CreationInfo section of the document as the VEX author.
In the same way, when a VEX relationship does not have a created property,
the document's date must be considered as authoritative.""" ;
    rdfs:subClassOf security:VulnAssessmentRelationship ;
    ns0:term_status "Stable" ;
    sh:property [ sh:datatype xsd:string ;
            sh:maxCount 1 ;
            sh:name "vexVersion" ;
            sh:path security:vexVersion ],
        [ sh:datatype xsd:string ;
            sh:maxCount 1 ;
            sh:name "statusNotes" ;
            sh:path security:statusNotes ] .

software:SoftwareDependencyLinkType a owl:Class ;
    rdfs:comment "TODO" ;
    owl:oneOf ( <https://spdx.org/rdf/v3/Software/SoftwareDependencyLinkType/static> <https://spdx.org/rdf/v3/Software/SoftwareDependencyLinkType/dynamic> <https://spdx.org/rdf/v3/Software/SoftwareDependencyLinkType/other> <https://spdx.org/rdf/v3/Software/SoftwareDependencyLinkType/tool> ) ;
    ns0:term_status "Stable" .

core:ExternalIdentifier a owl:Class,
        sh:NodeShape ;
    rdfs:comment """An ExternalIdentifier is a reference to a resource outside the scope of SPDX-3.0 content
that uniquely identifies an Element.""" ;
    ns0:term_status "Stable" ;
    sh:property [ sh:datatype xsd:anyURI ;
            sh:name "identifierLocator" ;
            sh:path core:identifierLocator ],
        [ sh:datatype xsd:string ;
            sh:maxCount 1 ;
            sh:name "comment" ;
            sh:path core:comment ],
        [ sh:datatype xsd:string ;
            sh:maxCount 1 ;
            sh:minCount 1 ;
            sh:name "identifier" ;
            sh:path core:identifier ],
        [ sh:datatype xsd:anyURI ;
            sh:maxCount 1 ;
            sh:name "issuingAuthority" ;
            sh:path core:issuingAuthority ],
        [ sh:class core:ExternalIdentifierType ;
            sh:maxCount 1 ;
            sh:minCount 1 ;
            sh:name "externalIdentifierType" ;
            sh:path core:externalIdentifierType ] .

dataset:DatasetAvailabilityType a owl:Class ;
    rdfs:comment "Describes the possible types of availability of a dataset, indicating whether the dataset can be directly downloaded, can be assembled using a script for scraping the data, is only available after a clickthrough or a registration form." ;
    owl:oneOf ( <https://spdx.org/rdf/v3/Dataset/DatasetAvailabilityType/query> <https://spdx.org/rdf/v3/Dataset/DatasetAvailabilityType/directDownload> <https://spdx.org/rdf/v3/Dataset/DatasetAvailabilityType/clickthrough> <https://spdx.org/rdf/v3/Dataset/DatasetAvailabilityType/registration> <https://spdx.org/rdf/v3/Dataset/DatasetAvailabilityType/scrapingScript> ) ;
    ns0:term_status "Stable" .

security:VexJustificationType a owl:Class ;
    rdfs:comment "VexJustificationType specifies the type of Vulnerability Exploitability eXchange (VEX) justification." ;
    owl:oneOf ( <https://spdx.org/rdf/v3/Security/VexJustificationType/inlineMitigationsAlreadyExist> <https://spdx.org/rdf/v3/Security/VexJustificationType/vulnerableCodeCannotBeControlledByAdversary> <https://spdx.org/rdf/v3/Security/VexJustificationType/vulnerableCodeNotInExecutePath> <https://spdx.org/rdf/v3/Security/VexJustificationType/componentNotPresent> <https://spdx.org/rdf/v3/Security/VexJustificationType/vulnerableCodeNotPresent> ) ;
    ns0:term_status "Stable" .

software:DependencyConditionalityType a owl:Class ;
    rdfs:comment "TODO" ;
    owl:oneOf ( <https://spdx.org/rdf/v3/Software/DependencyConditionalityType/provided> <https://spdx.org/rdf/v3/Software/DependencyConditionalityType/prerequisite> <https://spdx.org/rdf/v3/Software/DependencyConditionalityType/optional> <https://spdx.org/rdf/v3/Software/DependencyConditionalityType/required> <https://spdx.org/rdf/v3/Software/DependencyConditionalityType/other> ) ;
    ns0:term_status "Stable" .

software:Package a owl:Class,
        sh:NodeShape ;
    rdfs:comment """A package refers to any unit of content that can be associated with a distribution of software.
Typically, a package is composed of one or more files.  
Any of the following non-limiting examples may be (but are not required to be) represented in SPDX as a package:

 - a tarball, zip file or other archive
 - a directory or sub-directory
 - a separately distributed piece of software which another Package or File uses or depends upon (e.g., a Python package, a Go module, ...)
 - a container image, and/or each image layer within a container image
 - a collection of one or more sub-packages
 - a Git repository snapshot from a particular point in time

Note that some of these could be represented in SPDX as a file as well.
External property restriction on /Core/Element/name: minCount: 1""" ;
    rdfs:subClassOf software:SoftwareArtifact ;
    ns0:term_status "Stable" ;
    sh:property [ sh:datatype xsd:string ;
            sh:maxCount 1 ;
            sh:name "packageVersion" ;
            sh:path software:packageVersion ],
        [ sh:datatype xsd:string ;
            sh:maxCount 1 ;
            sh:name "sourceInfo" ;
            sh:path software:sourceInfo ],
        [ sh:datatype xsd:anyURI ;
            sh:maxCount 1 ;
            sh:name "downloadLocation" ;
            sh:path software:downloadLocation ],
        [ sh:datatype xsd:anyURI ;
            sh:maxCount 1 ;
            sh:name "packageUrl" ;
            sh:path software:packageUrl ],
        [ sh:datatype xsd:anyURI ;
            sh:maxCount 1 ;
            sh:name "homePage" ;
            sh:path software:homePage ] .

core:CreationInfo a owl:Class,
        sh:NodeShape ;
    rdfs:comment """The CreationInfo provides information about who created the Element, and when and how it was created. 

The dateTime created is often the date of last change (e.g., a git commit date), not the date when the SPDX data was created, as doing so supports reproducible builds.""" ;
    ns0:term_status "Stable" ;
    sh:property [ sh:datatype xsd:string ;
            sh:maxCount 1 ;
            sh:minCount 1 ;
            sh:name "dataLicense" ;
            sh:path core:dataLicense ],
        [ sh:datatype core:SemVer ;
            sh:maxCount 1 ;
            sh:minCount 1 ;
            sh:name "specVersion" ;
            sh:path core:specVersion ],
        [ sh:class core:Tool ;
            sh:name "createdUsing" ;
            sh:path core:createdUsing ],
        [ sh:class core:Agent ;
            sh:minCount 1 ;
            sh:name "createdBy" ;
            sh:path core:createdBy ],
        [ sh:datatype xsd:string ;
            sh:maxCount 1 ;
            sh:name "comment" ;
            sh:path core:comment ],
        [ sh:datatype core:DateTime ;
            sh:maxCount 1 ;
            sh:minCount 1 ;
            sh:name "created" ;
            sh:path core:created ] .

core:LifecycleScopeType a owl:Class ;
    rdfs:comment "TODO" ;
    owl:oneOf ( <https://spdx.org/rdf/v3/Core/LifecycleScopeType/other> <https://spdx.org/rdf/v3/Core/LifecycleScopeType/runtime> <https://spdx.org/rdf/v3/Core/LifecycleScopeType/test> <https://spdx.org/rdf/v3/Core/LifecycleScopeType/design> <https://spdx.org/rdf/v3/Core/LifecycleScopeType/development> <https://spdx.org/rdf/v3/Core/LifecycleScopeType/build> ) ;
    ns0:term_status "Stable" .

core:Relationship a owl:Class,
        sh:NodeShape ;
    rdfs:comment """A Relationship is a grouping of characteristics unique to an assertion
that one Element is related to one or more other Elements in some way.""" ;
    rdfs:subClassOf core:Element ;
    ns0:term_status "Stable" ;
    sh:property [ sh:datatype core:DateTime ;
            sh:maxCount 1 ;
            sh:name "endTime" ;
            sh:path core:endTime ],
        [ sh:datatype core:DateTime ;
            sh:maxCount 1 ;
            sh:name "startTime" ;
            sh:path core:startTime ],
        [ sh:class core:RelationshipCompleteness ;
            sh:maxCount 1 ;
            sh:name "completeness" ;
            sh:path core:completeness ],
        [ sh:class core:RelationshipType ;
            sh:maxCount 1 ;
            sh:minCount 1 ;
            sh:name "relationshipType" ;
            sh:path core:relationshipType ],
        [ sh:class core:Element ;
            sh:maxCount 1 ;
            sh:minCount 1 ;
            sh:name "from" ;
            sh:path core:from ],
        [ sh:class core:Element ;
            sh:name "to" ;
            sh:path core:to ] .

security:CvssSeverityType a owl:Class ;
    rdfs:comment "CvssSeverityType specifies the CVSS severity type, defined in the CVSS specifications as the textual representation of the numeric CVSS score. The severity type entries are inclusive of and applicable to enumerations found in CVSS versions [3](https://www.first.org/cvss/v3.0/specification-document#Qualitative-Severity-Rating-Scale) and [4](https://www.first.org/cvss/v4.0/specification-document#Qualitative-Severity-Rating-Scale). CvssSeverityType is a mandatory field because baseSeverity is required in the CVSS version [3.0](https://www.first.org/cvss/cvss-v3.0.json), [3.1](https://www.first.org/cvss/cvss-v3.1.json), and [4.0](https://www.first.org/cvss/cvss-v4.0.json) schemas. The field can be used to document the base, temporal, threat, or environmental severity." ;
    owl:oneOf ( <https://spdx.org/rdf/v3/Security/CvssSeverityType/low> <https://spdx.org/rdf/v3/Security/CvssSeverityType/high> <https://spdx.org/rdf/v3/Security/CvssSeverityType/none> <https://spdx.org/rdf/v3/Security/CvssSeverityType/medium> <https://spdx.org/rdf/v3/Security/CvssSeverityType/critical> ) ;
    ns0:term_status "Stable" .

simplelicensing:AnyLicenseInfo a owl:Class,
        sh:NodeShape ;
    rdfs:comment """An AnyLicenseInfo is used by licensing properties of software artifacts.
It can be a NoneLicense, a NoAssertionLicense,
single license (either on the SPDX License List or a custom-defined license);
a single license with an "or later" operator applied; the foregoing with
additional text applied; or a set of licenses combined by applying "AND" and
"OR" operators recursively.""" ;
    rdfs:subClassOf core:Element ;
    ns0:term_status "Stable" .

software:SbomType a owl:Class ;
    rdfs:comment """The set of SBOM types with definitions as defined in [Types of Software Bill of Material (SBOM) Documents](https://www.cisa.gov/sites/default/files/2023-04/sbom-types-document-508c.pdf), published on April 21, 2023. 
An SBOM type describes the most likely type of an SBOM from the producer perspective, so that consumers can draw conclusions about the data inside an SBOM.  A single SBOM can have multiple SBOM document types associated with it.""" ;
    owl:oneOf ( <https://spdx.org/rdf/v3/Software/SbomType/runtime> <https://spdx.org/rdf/v3/Software/SbomType/deployed> <https://spdx.org/rdf/v3/Software/SbomType/source> <https://spdx.org/rdf/v3/Software/SbomType/analyzed> <https://spdx.org/rdf/v3/Software/SbomType/build> <https://spdx.org/rdf/v3/Software/SbomType/design> ) ;
    ns0:term_status "Stable" .

software:SoftwareArtifact a owl:Class,
        sh:NodeShape ;
    rdfs:comment """A software artifact is a distinct article or unit related to software
such as a package, a file, or a snippet.""" ;
    rdfs:subClassOf core:Artifact ;
    ns0:term_status "Stable" ;
    sh:property [ sh:datatype xsd:string ;
            sh:maxCount 1 ;
            sh:name "copyrightText" ;
            sh:path software:copyrightText ],
        [ sh:datatype xsd:string ;
            sh:name "attributionText" ;
            sh:path software:attributionText ],
        [ sh:class software:SoftwarePurpose ;
            sh:maxCount 1 ;
            sh:name "primaryPurpose" ;
            sh:path software:primaryPurpose ],
        [ sh:datatype xsd:anyURI ;
            sh:maxCount 1 ;
            sh:name "contentIdentifier" ;
            sh:path software:contentIdentifier ],
        [ sh:class software:SoftwarePurpose ;
            sh:name "additionalPurpose" ;
            sh:path software:additionalPurpose ] .

build:Build a owl:Class,
        sh:NodeShape ;
    rdfs:comment """A build is a representation of the process in which a piece of software or artifact is built. It encapsulates information related to a build process and
provides an element from which relationships can be created to describe the build's inputs, outputs, and related entities (e.g. builders, identities, etc.).

Definitions of "BuildType", "ConfigSource", "Parameters" and "Environment" follow
those defined in [SLSA provenance](https://slsa.dev/provenance/v0.2).

ExternalIdentifier of type "urlScheme" may be used to identify build logs. In this case, the comment of the ExternalIdentifier should be "LogReference".

Note that buildStart and buildEnd are optional, and may be omitted to simplify creating reproducible builds.""" ;
    rdfs:subClassOf core:Element ;
    ns0:term_status "Stable" ;
    sh:property [ sh:class core:Hash ;
            sh:name "configSourceDigest" ;
            sh:path build:configSourceDigest ],
        [ sh:datatype core:DateTime ;
            sh:maxCount 1 ;
            sh:name "buildEndTime" ;
            sh:path build:buildEndTime ],
        [ sh:class core:DictionaryEntry ;
            sh:name "parameters" ;
            sh:path build:parameters ],
        [ sh:datatype xsd:anyURI ;
            sh:name "configSourceUri" ;
            sh:path build:configSourceUri ],
        [ sh:datatype xsd:string ;
            sh:maxCount 1 ;
            sh:name "buildId" ;
            sh:path build:buildId ],
        [ sh:datatype core:DateTime ;
            sh:maxCount 1 ;
            sh:name "buildStartTime" ;
            sh:path build:buildStartTime ],
        [ sh:datatype xsd:string ;
            sh:name "configSourceEntrypoint" ;
            sh:path build:configSourceEntrypoint ],
        [ sh:datatype xsd:anyURI ;
            sh:maxCount 1 ;
            sh:minCount 1 ;
            sh:name "buildType" ;
            sh:path build:buildType ],
        [ sh:class core:DictionaryEntry ;
            sh:name "environment" ;
            sh:path build:environment ] .

core:PresenceType a owl:Class ;
    rdfs:comment "This type is used to indicate if a given field is present or absent or unknown." ;
    owl:oneOf ( <https://spdx.org/rdf/v3/Core/PresenceType/noAssertion> <https://spdx.org/rdf/v3/Core/PresenceType/yes> <https://spdx.org/rdf/v3/Core/PresenceType/no> ) ;
    ns0:term_status "Stable" .

expandedlicensing:LicenseAddition a owl:Class,
        sh:NodeShape ;
    rdfs:comment """A LicenseAddition represents text which is intended to be added to a License
as additional text, but which is not itself intended to be a standalone
License.

It may be an exception which is listed on the SPDX Exceptions List
(ListedLicenseException), or may be any other additional text (as an exception
or otherwise) which is defined by an SPDX data creator (CustomLicenseAddition).""" ;
    rdfs:subClassOf core:Element ;
    ns0:term_status "Stable" ;
    sh:property [ sh:datatype xsd:string ;
            sh:maxCount 1 ;
            sh:name "licenseXml" ;
            sh:path expandedlicensing:licenseXml ],
        [ sh:datatype xsd:string ;
            sh:maxCount 1 ;
            sh:name "obsoletedBy" ;
            sh:path expandedlicensing:obsoletedBy ],
        [ sh:datatype xsd:string ;
            sh:maxCount 1 ;
            sh:name "standardAdditionTemplate" ;
            sh:path expandedlicensing:standardAdditionTemplate ],
        [ sh:datatype xsd:boolean ;
            sh:maxCount 1 ;
            sh:name "isDeprecatedAdditionId" ;
            sh:path expandedlicensing:isDeprecatedAdditionId ],
        [ sh:datatype xsd:string ;
            sh:maxCount 1 ;
            sh:minCount 1 ;
            sh:name "additionText" ;
            sh:path expandedlicensing:additionText ] .

core:Artifact a owl:Class,
        sh:NodeShape ;
    rdfs:comment """An artifact is a distinct article or unit within the digital domain,
such as an electronic file, a software package, a device or an element of data.""" ;
    rdfs:subClassOf core:Element ;
    ns0:term_status "Stable" ;
    sh:property [ sh:class core:Agent ;
            sh:name "originatedBy" ;
            sh:path core:originatedBy ],
        [ sh:class core:Agent ;
            sh:maxCount 1 ;
            sh:name "suppliedBy" ;
            sh:path core:suppliedBy ],
        [ sh:datatype core:DateTime ;
            sh:maxCount 1 ;
            sh:name "releaseTime" ;
            sh:path core:releaseTime ],
        [ sh:datatype core:DateTime ;
            sh:maxCount 1 ;
            sh:name "builtTime" ;
            sh:path core:builtTime ],
        [ sh:datatype core:DateTime ;
            sh:maxCount 1 ;
            sh:name "validUntilTime" ;
            sh:path core:validUntilTime ],
        [ sh:datatype xsd:string ;
            sh:name "standard" ;
            sh:path core:standard ] .

core:Agent a owl:Class,
        sh:NodeShape ;
    rdfs:comment "The Agent class represents anything that has the potential to act on a system. This could be a person, organization, software agent, etc. This is not to be confused with tools that are used to perform tasks." ;
    rdfs:subClassOf core:Element ;
    ns0:term_status "Stable" .

expandedlicensing:License a owl:Class,
        sh:NodeShape ;
    rdfs:comment """A License represents a license text, whether listed on the SPDX License List
(ListedLicense) or defined by an SPDX data creator (CustomLicense).""" ;
    rdfs:subClassOf expandedlicensing:ExtendableLicense ;
    ns0:term_status "Stable" ;
    sh:property [ sh:datatype xsd:boolean ;
            sh:maxCount 1 ;
            sh:name "isOsiApproved" ;
            sh:path expandedlicensing:isOsiApproved ],
        [ sh:datatype xsd:string ;
            sh:maxCount 1 ;
            sh:name "standardLicenseTemplate" ;
            sh:path expandedlicensing:standardLicenseTemplate ],
        [ sh:datatype xsd:boolean ;
            sh:maxCount 1 ;
            sh:name "isDeprecatedLicenseId" ;
            sh:path expandedlicensing:isDeprecatedLicenseId ],
        [ sh:datatype xsd:string ;
            sh:maxCount 1 ;
            sh:minCount 1 ;
            sh:name "/SimpleLicensing/licenseText" ;
            sh:path simplelicensing:licenseText ],
        [ sh:datatype xsd:boolean ;
            sh:maxCount 1 ;
            sh:name "isFsfLibre" ;
            sh:path expandedlicensing:isFsfLibre ],
        [ sh:datatype xsd:string ;
            sh:maxCount 1 ;
            sh:name "standardLicenseHeader" ;
            sh:path expandedlicensing:standardLicenseHeader ],
        [ sh:datatype xsd:string ;
            sh:maxCount 1 ;
            sh:name "licenseXml" ;
            sh:path expandedlicensing:licenseXml ],
        [ sh:datatype xsd:string ;
            sh:maxCount 1 ;
            sh:name "obsoletedBy" ;
            sh:path expandedlicensing:obsoletedBy ] .

core:ProfileIdentifierType a owl:Class ;
    rdfs:comment """There are a set of profiles that have been defined by a profile team.
A profile consists of a namespace that may add properties and classes to the core profile unique to the domain covered by the profile.
The profile may also contain additional restrictions on existing properties and classes defined in other profiles.
If the creator of an SPDX collection of elements includes a profile in the list of conformanceProfiles, they are claiming that all contained elements conform to all restrictions defined for that profile.""" ;
    owl:oneOf ( <https://spdx.org/rdf/v3/Core/ProfileIdentifierType/build> <https://spdx.org/rdf/v3/Core/ProfileIdentifierType/usage> <https://spdx.org/rdf/v3/Core/ProfileIdentifierType/dataset> <https://spdx.org/rdf/v3/Core/ProfileIdentifierType/core> <https://spdx.org/rdf/v3/Core/ProfileIdentifierType/ai> <https://spdx.org/rdf/v3/Core/ProfileIdentifierType/simpleLicensing> <https://spdx.org/rdf/v3/Core/ProfileIdentifierType/software> <https://spdx.org/rdf/v3/Core/ProfileIdentifierType/extension> <https://spdx.org/rdf/v3/Core/ProfileIdentifierType/security> <https://spdx.org/rdf/v3/Core/ProfileIdentifierType/expandedLicensing> ) ;
    ns0:term_status "Stable" .

security:VulnAssessmentRelationship a owl:Class,
        sh:NodeShape ;
    rdfs:comment """VulnAssessmentRelationship is the ancestor class common to all vulnerability
assessment relationships. It factors out the common properties shared by them.
External property restriction on /Core/Relationship/to: minCount: 1""" ;
    rdfs:subClassOf core:Relationship ;
    ns0:term_status "Stable" ;
    sh:property [ sh:datatype core:DateTime ;
            sh:maxCount 1 ;
            sh:name "publishedTime" ;
            sh:path security:publishedTime ],
        [ sh:class core:Agent ;
            sh:maxCount 1 ;
            sh:name "suppliedBy" ;
            sh:path security:suppliedBy ],
        [ sh:class core:Element ;
            sh:maxCount 1 ;
            sh:name "assessedElement" ;
            sh:path security:assessedElement ],
        [ sh:datatype core:DateTime ;
            sh:maxCount 1 ;
            sh:name "modifiedTime" ;
            sh:path security:modifiedTime ],
        [ sh:datatype core:DateTime ;
            sh:maxCount 1 ;
            sh:name "withdrawnTime" ;
            sh:path security:withdrawnTime ] .

core:ExternalIdentifierType a owl:Class ;
    rdfs:comment "ExteralIdentifierType specifies the type of an external identifier." ;
    owl:oneOf ( <https://spdx.org/rdf/v3/Core/ExternalIdentifierType/swhid> <https://spdx.org/rdf/v3/Core/ExternalIdentifierType/other> <https://spdx.org/rdf/v3/Core/ExternalIdentifierType/urlScheme> <https://spdx.org/rdf/v3/Core/ExternalIdentifierType/cve> <https://spdx.org/rdf/v3/Core/ExternalIdentifierType/cpe23> <https://spdx.org/rdf/v3/Core/ExternalIdentifierType/swid> <https://spdx.org/rdf/v3/Core/ExternalIdentifierType/cpe22> <https://spdx.org/rdf/v3/Core/ExternalIdentifierType/pkgUrl> <https://spdx.org/rdf/v3/Core/ExternalIdentifierType/gitoid> <https://spdx.org/rdf/v3/Core/ExternalIdentifierType/email> <https://spdx.org/rdf/v3/Core/ExternalIdentifierType/securityOther> ) ;
    ns0:term_status "Stable" .

dataset:Dataset a owl:Class,
        sh:NodeShape ;
    rdfs:comment """Metadata information that can be added to a dataset that may be used in a software or to train/test an AI package.
External property restriction on /Core/Artifact/originatedBy: minCount: 1
External property restriction on /Software/Package/downloadLocation: minCount: 1
External property restriction on /Software/SoftwareArtifact/primaryPurpose: minCount: 1
External property restriction on /Core/Artifact/releaseTime: minCount: 1
External property restriction on /Core/Artifact/builtTime: minCount: 1""" ;
    rdfs:subClassOf software:Package ;
    ns0:term_status "Stable" ;
    sh:property [ sh:datatype xsd:string ;
            sh:name "anonymizationMethodUsed" ;
            sh:path dataset:anonymizationMethodUsed ],
        [ sh:datatype xsd:nonNegativeInteger ;
            sh:maxCount 1 ;
            sh:name "datasetSize" ;
            sh:path dataset:datasetSize ],
        [ sh:class core:PresenceType ;
            sh:maxCount 1 ;
            sh:name "sensitivePersonalInformation" ;
            sh:path dataset:sensitivePersonalInformation ],
        [ sh:class dataset:DatasetType ;
            sh:minCount 1 ;
            sh:name "datasetType" ;
            sh:path dataset:datasetType ],
        [ sh:datatype xsd:string ;
            sh:maxCount 1 ;
            sh:name "datasetUpdateMechanism" ;
            sh:path dataset:datasetUpdateMechanism ],
        [ sh:datatype xsd:string ;
            sh:name "knownBias" ;
            sh:path dataset:knownBias ],
        [ sh:class dataset:DatasetAvailabilityType ;
            sh:maxCount 1 ;
            sh:name "datasetAvailability" ;
            sh:path dataset:datasetAvailability ],
        [ sh:class dataset:ConfidentialityLevelType ;
            sh:maxCount 1 ;
            sh:name "confidentialityLevel" ;
            sh:path dataset:confidentialityLevel ],
        [ sh:datatype xsd:string ;
            sh:maxCount 1 ;
            sh:name "intendedUse" ;
            sh:path dataset:intendedUse ],
        [ sh:datatype xsd:string ;
            sh:maxCount 1 ;
            sh:name "datasetNoise" ;
            sh:path dataset:datasetNoise ],
        [ sh:datatype xsd:string ;
            sh:maxCount 1 ;
            sh:name "dataCollectionProcess" ;
            sh:path dataset:dataCollectionProcess ],
        [ sh:datatype xsd:string ;
            sh:name "dataPreprocessing" ;
            sh:path dataset:dataPreprocessing ],
        [ sh:class core:DictionaryEntry ;
            sh:name "sensor" ;
            sh:path dataset:sensor ] .

ai:AIPackage a owl:Class,
        sh:NodeShape ;
    rdfs:comment """Metadata information that can be added to a package to describe an AI application or trained AI model.
External property restriction on /Core/Artifact/suppliedBy: minCount: 1
External property restriction on /Software/Package/downloadLocation: minCount: 1
External property restriction on /Software/Package/packageVersion: minCount: 1
External property restriction on /Software/SoftwareArtifact/primaryPurpose: minCount: 1
External property restriction on /Core/Artifact/releaseTime: minCount: 1""" ;
    rdfs:subClassOf software:Package ;
    ns0:term_status "Stable" ;
    sh:property [ sh:datatype xsd:string ;
            sh:maxCount 1 ;
            sh:name "informationAboutApplication" ;
            sh:path ai:informationAboutApplication ],
        [ sh:datatype xsd:string ;
            sh:maxCount 1 ;
            sh:name "informationAboutTraining" ;
            sh:path ai:informationAboutTraining ],
        [ sh:class core:PresenceType ;
            sh:maxCount 1 ;
            sh:name "sensitivePersonalInformation" ;
            sh:path ai:sensitivePersonalInformation ],
        [ sh:datatype xsd:string ;
            sh:name "modelDataPreprocessing" ;
            sh:path ai:modelDataPreprocessing ],
        [ sh:datatype xsd:string ;
            sh:name "modelExplainability" ;
            sh:path ai:modelExplainability ],
        [ sh:datatype xsd:string ;
            sh:name "standardCompliance" ;
            sh:path ai:standardCompliance ],
        [ sh:class core:PresenceType ;
            sh:maxCount 1 ;
            sh:name "autonomyType" ;
            sh:path ai:autonomyType ],
        [ sh:class core:DictionaryEntry ;
            sh:name "hyperparameter" ;
            sh:path ai:hyperparameter ],
        [ sh:class ai:SafetyRiskAssessmentType ;
            sh:maxCount 1 ;
            sh:name "safetyRiskAssessment" ;
            sh:path ai:safetyRiskAssessment ],
        [ sh:class core:DictionaryEntry ;
            sh:name "metric" ;
            sh:path ai:metric ],
        [ sh:datatype xsd:string ;
            sh:maxCount 1 ;
            sh:name "energyConsumption" ;
            sh:path ai:energyConsumption ],
        [ sh:datatype xsd:string ;
            sh:maxCount 1 ;
            sh:name "limitation" ;
            sh:path ai:limitation ],
        [ sh:datatype xsd:string ;
            sh:name "domain" ;
            sh:path ai:domain ],
        [ sh:datatype xsd:string ;
            sh:name "typeOfModel" ;
            sh:path ai:typeOfModel ],
        [ sh:class core:DictionaryEntry ;
            sh:name "metricDecisionThreshold" ;
            sh:path ai:metricDecisionThreshold ] .

core:DictionaryEntry a owl:Class,
        sh:NodeShape ;
    rdfs:comment "The class used for implementing a generic string mapping (also known as associative array, dictionary, or hash map) in SPDX.  Each DictionaryEntry contains a key-value pair which maps the key to its associated value.  To implement a dictionary, this class is to be used in a collection with unique keys." ;
    ns0:term_status "Stable" ;
    sh:property [ sh:datatype xsd:string ;
            sh:maxCount 1 ;
            sh:name "value" ;
            sh:path core:value ],
        [ sh:datatype xsd:string ;
            sh:maxCount 1 ;
            sh:minCount 1 ;
            sh:name "key" ;
            sh:path core:key ] .

dataset:DatasetType a owl:Class ;
    rdfs:comment "Describes the different structures of data within a given dataset. A dataset can have multiple types of data, or even a single type of data but still match multiple types, for example sensor data could also be timeseries or labeled image data could also be considered categorical." ;
    owl:oneOf ( <https://spdx.org/rdf/v3/Dataset/DatasetType/categorical> <https://spdx.org/rdf/v3/Dataset/DatasetType/syntactic> <https://spdx.org/rdf/v3/Dataset/DatasetType/text> <https://spdx.org/rdf/v3/Dataset/DatasetType/sensor> <https://spdx.org/rdf/v3/Dataset/DatasetType/video> <https://spdx.org/rdf/v3/Dataset/DatasetType/audio> <https://spdx.org/rdf/v3/Dataset/DatasetType/structured> <https://spdx.org/rdf/v3/Dataset/DatasetType/timestamp> <https://spdx.org/rdf/v3/Dataset/DatasetType/image> <https://spdx.org/rdf/v3/Dataset/DatasetType/other> <https://spdx.org/rdf/v3/Dataset/DatasetType/noAssertion> <https://spdx.org/rdf/v3/Dataset/DatasetType/numeric> <https://spdx.org/rdf/v3/Dataset/DatasetType/timeseries> <https://spdx.org/rdf/v3/Dataset/DatasetType/graph> ) ;
    ns0:term_status "Stable" .

core:HashAlgorithm a owl:Class ;
    rdfs:comment """A HashAlgorithm is a mathematical algorithm that maps data of arbitrary size to a bit string (the hash)
and is a one-way function, that is, a function which is practically infeasible to invert.""" ;
    owl:oneOf ( <https://spdx.org/rdf/v3/Core/HashAlgorithm/blake2b512> <https://spdx.org/rdf/v3/Core/HashAlgorithm/sha512> <https://spdx.org/rdf/v3/Core/HashAlgorithm/md5> <https://spdx.org/rdf/v3/Core/HashAlgorithm/spdxPvcSha256> <https://spdx.org/rdf/v3/Core/HashAlgorithm/spdxPvcSha1> <https://spdx.org/rdf/v3/Core/HashAlgorithm/sha1> <https://spdx.org/rdf/v3/Core/HashAlgorithm/sha256> <https://spdx.org/rdf/v3/Core/HashAlgorithm/blake2b384> <https://spdx.org/rdf/v3/Core/HashAlgorithm/sha3_384> <https://spdx.org/rdf/v3/Core/HashAlgorithm/crystalsDilithium> <https://spdx.org/rdf/v3/Core/HashAlgorithm/falcon> <https://spdx.org/rdf/v3/Core/HashAlgorithm/blake2b256> <https://spdx.org/rdf/v3/Core/HashAlgorithm/md6> <https://spdx.org/rdf/v3/Core/HashAlgorithm/blake3> <https://spdx.org/rdf/v3/Core/HashAlgorithm/sha3_224> <https://spdx.org/rdf/v3/Core/HashAlgorithm/sphincsPlus> <https://spdx.org/rdf/v3/Core/HashAlgorithm/sha384> <https://spdx.org/rdf/v3/Core/HashAlgorithm/md4> <https://spdx.org/rdf/v3/Core/HashAlgorithm/sha3_512> <https://spdx.org/rdf/v3/Core/HashAlgorithm/sha224> <https://spdx.org/rdf/v3/Core/HashAlgorithm/md2> <https://spdx.org/rdf/v3/Core/HashAlgorithm/other> <https://spdx.org/rdf/v3/Core/HashAlgorithm/crystalsKyber> <https://spdx.org/rdf/v3/Core/HashAlgorithm/sha3_256> ) ;
    ns0:term_status "Stable" .

core:Element a owl:Class,
        sh:NodeShape ;
    rdfs:comment """An Element is a representation of a fundamental concept either directly inherent
to the Bill of Materials (BOM) domain or indirectly related to the BOM domain
and necessary for contextually characterizing BOM concepts and relationships.
Within SPDX-3.0 structure this is the base class acting as a consistent,
unifying, and interoperable foundation for all explicit
and inter-relatable content objects.""" ;
    rdfs:subClassOf owl:Thing ;
    ns0:term_status "Stable" ;
    sh:property [ sh:class core:CreationInfo ;
            sh:maxCount 1 ;
            sh:minCount 1 ;
            sh:name "creationInfo" ;
            sh:path core:creationInfo ],
        [ sh:datatype xsd:string ;
            sh:maxCount 1 ;
            sh:name "comment" ;
            sh:path core:comment ],
        [ sh:datatype core:Extension ;
            sh:name "extension" ;
            sh:path core:extension ],
        [ sh:datatype xsd:string ;
            sh:maxCount 1 ;
            sh:name "description" ;
            sh:path core:description ],
        [ sh:class core:ExternalIdentifier ;
            sh:name "externalIdentifier" ;
            sh:path core:externalIdentifier ],
        [ sh:datatype xsd:string ;
            sh:maxCount 1 ;
            sh:name "name" ;
            sh:path core:name ],
        [ sh:class core:ExternalRef ;
            sh:name "externalRef" ;
            sh:path core:externalRef ],
        [ sh:class core:IntegrityMethod ;
            sh:name "verifiedUsing" ;
            sh:path core:verifiedUsing ],
        [ sh:datatype xsd:string ;
            sh:maxCount 1 ;
            sh:name "summary" ;
            sh:path core:summary ] .

software:SoftwarePurpose a owl:Class ;
    rdfs:comment """This field provides information about the primary purpose of an Element.
Software Purpose is intrinsic to how the Element is being used rather than the content of the Element.
This field is a reasonable estimate of the most likely usage of the Element
from the producer and consumer perspective from which both parties can draw conclusions
about the context in which the Element exists.""" ;
    owl:oneOf ( <https://spdx.org/rdf/v3/Software/SoftwarePurpose/specification> <https://spdx.org/rdf/v3/Software/SoftwarePurpose/firmware> <https://spdx.org/rdf/v3/Software/SoftwarePurpose/install> <https://spdx.org/rdf/v3/Software/SoftwarePurpose/library> <https://spdx.org/rdf/v3/Software/SoftwarePurpose/file> <https://spdx.org/rdf/v3/Software/SoftwarePurpose/test> <https://spdx.org/rdf/v3/Software/SoftwarePurpose/module> <https://spdx.org/rdf/v3/Software/SoftwarePurpose/data> <https://spdx.org/rdf/v3/Software/SoftwarePurpose/requirement> <https://spdx.org/rdf/v3/Software/SoftwarePurpose/source> <https://spdx.org/rdf/v3/Software/SoftwarePurpose/framework> <https://spdx.org/rdf/v3/Software/SoftwarePurpose/archive> <https://spdx.org/rdf/v3/Software/SoftwarePurpose/device> <https://spdx.org/rdf/v3/Software/SoftwarePurpose/deviceDriver> <https://spdx.org/rdf/v3/Software/SoftwarePurpose/container> <https://spdx.org/rdf/v3/Software/SoftwarePurpose/bom> <https://spdx.org/rdf/v3/Software/SoftwarePurpose/application> <https://spdx.org/rdf/v3/Software/SoftwarePurpose/other> <https://spdx.org/rdf/v3/Software/SoftwarePurpose/patch> <https://spdx.org/rdf/v3/Software/SoftwarePurpose/operatingSystem> <https://spdx.org/rdf/v3/Software/SoftwarePurpose/platform> <https://spdx.org/rdf/v3/Software/SoftwarePurpose/filesystemImage> <https://spdx.org/rdf/v3/Software/SoftwarePurpose/configuration> <https://spdx.org/rdf/v3/Software/SoftwarePurpose/evidence> <https://spdx.org/rdf/v3/Software/SoftwarePurpose/model> <https://spdx.org/rdf/v3/Software/SoftwarePurpose/manifest> <https://spdx.org/rdf/v3/Software/SoftwarePurpose/diskImage> <https://spdx.org/rdf/v3/Software/SoftwarePurpose/documentation> <https://spdx.org/rdf/v3/Software/SoftwarePurpose/executable> ) ;
    ns0:term_status "Stable" .

core:ExternalRefType a owl:Class ;
    rdfs:comment "ExternalRefType specifies the type of an external reference." ;
    owl:oneOf ( <https://spdx.org/rdf/v3/Core/ExternalRefType/funding> <https://spdx.org/rdf/v3/Core/ExternalRefType/eolNotice> <https://spdx.org/rdf/v3/Core/ExternalRefType/buildMeta> <https://spdx.org/rdf/v3/Core/ExternalRefType/npm> <https://spdx.org/rdf/v3/Core/ExternalRefType/staticAnalysisReport> <https://spdx.org/rdf/v3/Core/ExternalRefType/chat> <https://spdx.org/rdf/v3/Core/ExternalRefType/privacyAssessment> <https://spdx.org/rdf/v3/Core/ExternalRefType/binaryArtifact> <https://spdx.org/rdf/v3/Core/ExternalRefType/vcs> <https://spdx.org/rdf/v3/Core/ExternalRefType/componentAnalysisReport> <https://spdx.org/rdf/v3/Core/ExternalRefType/certificationReport> <https://spdx.org/rdf/v3/Core/ExternalRefType/securityAdversaryModel> <https://spdx.org/rdf/v3/Core/ExternalRefType/secureSoftwareAttestation> <https://spdx.org/rdf/v3/Core/ExternalRefType/mailingList> <https://spdx.org/rdf/v3/Core/ExternalRefType/securityPenTestReport> <https://spdx.org/rdf/v3/Core/ExternalRefType/sourceArtifact> <https://spdx.org/rdf/v3/Core/ExternalRefType/altWebPage> <https://spdx.org/rdf/v3/Core/ExternalRefType/bower> <https://spdx.org/rdf/v3/Core/ExternalRefType/runtimeAnalysisReport> <https://spdx.org/rdf/v3/Core/ExternalRefType/securityFix> <https://spdx.org/rdf/v3/Core/ExternalRefType/license> <https://spdx.org/rdf/v3/Core/ExternalRefType/securityPolicy> <https://spdx.org/rdf/v3/Core/ExternalRefType/vulnerabilityDisclosureReport> <https://spdx.org/rdf/v3/Core/ExternalRefType/mavenCentral> <https://spdx.org/rdf/v3/Core/ExternalRefType/securityThreatModel> <https://spdx.org/rdf/v3/Core/ExternalRefType/nuget> <https://spdx.org/rdf/v3/Core/ExternalRefType/releaseHistory> <https://spdx.org/rdf/v3/Core/ExternalRefType/vulnerabilityExploitabilityAssessment> <https://spdx.org/rdf/v3/Core/ExternalRefType/socialMedia> <https://spdx.org/rdf/v3/Core/ExternalRefType/exportControlAssessment> <https://spdx.org/rdf/v3/Core/ExternalRefType/dynamicAnalysisReport> <https://spdx.org/rdf/v3/Core/ExternalRefType/metrics> <https://spdx.org/rdf/v3/Core/ExternalRefType/securityAdvisory> <https://spdx.org/rdf/v3/Core/ExternalRefType/qualityAssessmentReport> <https://spdx.org/rdf/v3/Core/ExternalRefType/documentation> <https://spdx.org/rdf/v3/Core/ExternalRefType/support> <https://spdx.org/rdf/v3/Core/ExternalRefType/productMetadata> <https://spdx.org/rdf/v3/Core/ExternalRefType/purchaseOrder> <https://spdx.org/rdf/v3/Core/ExternalRefType/releaseNotes> <https://spdx.org/rdf/v3/Core/ExternalRefType/riskAssessment> <https://spdx.org/rdf/v3/Core/ExternalRefType/other> <https://spdx.org/rdf/v3/Core/ExternalRefType/buildSystem> <https://spdx.org/rdf/v3/Core/ExternalRefType/issueTracker> <https://spdx.org/rdf/v3/Core/ExternalRefType/securityOther> <https://spdx.org/rdf/v3/Core/ExternalRefType/altDownloadLocation> ) ;
    ns0:term_status "Stable" .

core:RelationshipType a owl:Class ;
    rdfs:comment """Provides information about the relationship between two Elements.
For example, you can represent a relationship between two different Files,
between a Package and a File, between two Packages, or between one SPDXDocument and another SPDXDocument.

Relationship names be descriptive enough to easily deduce the correct direction
from their name. The best way to do this is to make sure that the relationship
name completes the sentence:

`from` (is) (a) `RELATIONSHIP` `to`""" ;
    owl:oneOf ( <https://spdx.org/rdf/v3/Core/RelationshipType/hasExample> <https://spdx.org/rdf/v3/Core/RelationshipType/usesTool> <https://spdx.org/rdf/v3/Core/RelationshipType/underInvestigationFor> <https://spdx.org/rdf/v3/Core/RelationshipType/hasDocumentation> <https://spdx.org/rdf/v3/Core/RelationshipType/amendedBy> <https://spdx.org/rdf/v3/Core/RelationshipType/hasProvidedDependency> <https://spdx.org/rdf/v3/Core/RelationshipType/coordinatedBy> <https://spdx.org/rdf/v3/Core/RelationshipType/hasTest> <https://spdx.org/rdf/v3/Core/RelationshipType/hasMetadata> <https://spdx.org/rdf/v3/Core/RelationshipType/generates> <https://spdx.org/rdf/v3/Core/RelationshipType/hasDeclaredLicense> <https://spdx.org/rdf/v3/Core/RelationshipType/hasDeletedFile> <https://spdx.org/rdf/v3/Core/RelationshipType/hasOutputs> <https://spdx.org/rdf/v3/Core/RelationshipType/hasStaticLink> <https://spdx.org/rdf/v3/Core/RelationshipType/reportedBy> <https://spdx.org/rdf/v3/Core/RelationshipType/hasRequirement> <https://spdx.org/rdf/v3/Core/RelationshipType/hasAssociatedVulnerability> <https://spdx.org/rdf/v3/Core/RelationshipType/hasPrerequsite> <https://spdx.org/rdf/v3/Core/RelationshipType/hasVariant> <https://spdx.org/rdf/v3/Core/RelationshipType/descendantOf> <https://spdx.org/rdf/v3/Core/RelationshipType/hasEvidence> <https://spdx.org/rdf/v3/Core/RelationshipType/serializedInArtifact> <https://spdx.org/rdf/v3/Core/RelationshipType/configures> <https://spdx.org/rdf/v3/Core/RelationshipType/availableFrom> <https://spdx.org/rdf/v3/Core/RelationshipType/copiedTo> <https://spdx.org/rdf/v3/Core/RelationshipType/delegatedTo> <https://spdx.org/rdf/v3/Core/RelationshipType/hasHost> <https://spdx.org/rdf/v3/Core/RelationshipType/doesNotAffect> <https://spdx.org/rdf/v3/Core/RelationshipType/foundBy> <https://spdx.org/rdf/v3/Core/RelationshipType/exploitCreatedBy> <https://spdx.org/rdf/v3/Core/RelationshipType/hasInputs> <https://spdx.org/rdf/v3/Core/RelationshipType/describes> <https://spdx.org/rdf/v3/Core/RelationshipType/hasDependencyManifest> <https://spdx.org/rdf/v3/Core/RelationshipType/hasDataFile> <https://spdx.org/rdf/v3/Core/RelationshipType/dependsOn> <https://spdx.org/rdf/v3/Core/RelationshipType/hasDynamicLink> <https://spdx.org/rdf/v3/Core/RelationshipType/trainedOn> <https://spdx.org/rdf/v3/Core/RelationshipType/hasOptionalComponent> <https://spdx.org/rdf/v3/Core/RelationshipType/testedOn> <https://spdx.org/rdf/v3/Core/RelationshipType/hasSpecification> <https://spdx.org/rdf/v3/Core/RelationshipType/modifiedBy> <https://spdx.org/rdf/v3/Core/RelationshipType/hasDistributionArtifact> <https://spdx.org/rdf/v3/Core/RelationshipType/hasAddedFile> <https://spdx.org/rdf/v3/Core/RelationshipType/publishedBy> <https://spdx.org/rdf/v3/Core/RelationshipType/other> <https://spdx.org/rdf/v3/Core/RelationshipType/ancestorOf> <https://spdx.org/rdf/v3/Core/RelationshipType/expandsTo> <https://spdx.org/rdf/v3/Core/RelationshipType/contains> <https://spdx.org/rdf/v3/Core/RelationshipType/invokedBy> <https://spdx.org/rdf/v3/Core/RelationshipType/packagedBy> <https://spdx.org/rdf/v3/Core/RelationshipType/fixedIn> <https://spdx.org/rdf/v3/Core/RelationshipType/patchedBy> <https://spdx.org/rdf/v3/Core/RelationshipType/hasConcludedLicense> <https://spdx.org/rdf/v3/Core/RelationshipType/hasOptionalDependency> <https://spdx.org/rdf/v3/Core/RelationshipType/hasTestCase> <https://spdx.org/rdf/v3/Core/RelationshipType/affects> <https://spdx.org/rdf/v3/Core/RelationshipType/republishedBy> <https://spdx.org/rdf/v3/Core/RelationshipType/hasAssessmentFor> <https://spdx.org/rdf/v3/Core/RelationshipType/fixedBy> ) ;
    ns0:term_status "Stable" .

